Changed definitions and proofs so that the virtual memory is modeled as two party-indexed maps: one for each party's next available virtual address, and one for each party's virtual map. (Previously, it was modeled as two variables for each party, leading to duplication in code and assertions.)
Updated theREADME file.

Guessing.ec
@@ -155,20 +155,15 @@ module Memory : MEMORY = {
   var next_phys_addr : addr
   var phys_map : (addr, object) fmap
 
-  var honest_next_virt_addr : addr
-  var honest_virt_map    : (addr, addr) fmap
-
-  var malicious_next_virt_addr : addr
-  var malicious_virt_map : (addr, addr) fmap
+  var next_virt_addr : (party, addr) fmap
+  var virt_map : (party, (addr, addr) fmap) fmap
 
   proc init() : unit = {
-    next_key                 <- 0;
-    next_phys_addr           <- 0;
-    phys_map                 <- empty;
-    honest_next_virt_addr    <- 0;
-    honest_virt_map          <- empty;
-    malicious_next_virt_addr <- 0;
-    malicious_virt_map       <- empty;
+    next_key       <- 0;
+    next_phys_addr <- 0;
+    phys_map       <- empty;
+    next_virt_addr <- empty.[Honest <- 0].[Malicious <- 0];
+    virt_map       <- empty.[Honest <- empty].[Malicious <- empty];
   }
 
   proc phys_alloc(obj : object) : addr = {
@@ -179,41 +174,22 @@ module Memory : MEMORY = {
     return r;
   }
 
-  proc honest_virt_alloc(phys_addr : addr) : addr = {
-    var r : addr;
-    honest_virt_map.[honest_next_virt_addr] <- phys_addr;
-    r <- honest_next_virt_addr;
-    honest_next_virt_addr <- honest_next_virt_addr + 1;
-    return r;
-  }
-
-  proc malicious_virt_alloc(phys_addr : addr) : addr = {
-    var r : addr;
-    malicious_virt_map.[malicious_next_virt_addr] <- phys_addr;
-    r <- malicious_next_virt_addr;
-    malicious_next_virt_addr <- malicious_next_virt_addr + 1;
-    return r;
+  proc virt_alloc(pty : party, phys_addr : addr) : addr = {
+    var next : addr <- oget (next_virt_addr.[pty]);
+    virt_map.[pty] <- (oget virt_map.[pty]).[next <- phys_addr];
+    next_virt_addr.[pty] <- next + 1;
+    return next;
   }
 
   proc trans_virt_addr(pty : party, addr : addr) : addr option = {
     var r : addr option;
     var phys_addr, other_virt_addr : addr;
-    if (pty = Honest) {
-      if (addr \in honest_virt_map) {
-        phys_addr <- oget honest_virt_map.[addr];
-        other_virt_addr <@ malicious_virt_alloc(phys_addr);
-        r <- Some other_virt_addr;
-      }
-      else { r <- None; }
+    if (addr \in oget virt_map.[pty]) {
+      phys_addr <- oget (oget virt_map.[pty]).[addr];
+      other_virt_addr <@ virt_alloc(other pty, phys_addr);
+      r <- Some other_virt_addr;
     }
-    else {
-      if (addr \in malicious_virt_map) {
-        phys_addr <- oget malicious_virt_map.[addr];
-        other_virt_addr <@ honest_virt_alloc(phys_addr);
-        r <- Some other_virt_addr;
-      }
-      else { r <- None; }
-    }
+    else { r <- None; }
     return r;
   }
 
@@ -222,158 +198,83 @@ module Memory : MEMORY = {
     var phys_addr, virt_addr : addr;
     next_key <- next_key + 1;
     phys_addr <@ phys_alloc(Key key);
-    if (pty = Honest) {
-      virt_addr <@ honest_virt_alloc(phys_addr);
-    }
-    else {
-      virt_addr <@ malicious_virt_alloc(phys_addr);
-    }
+    virt_addr <@ virt_alloc(pty, phys_addr);
     return virt_addr;
   }
 
   proc is_key(pty : party, key_addr : addr) : bool = {
     var r : bool;
-    if (pty = Honest) {
-      if (key_addr \in honest_virt_map) {
-        r <- is_key (oget phys_map.[oget honest_virt_map.[key_addr]]);
-      }
-      else { r <- false; }
+    if (key_addr \in oget virt_map.[pty]) {
+      r <- is_key (oget phys_map.[oget (oget virt_map.[pty]).[key_addr]]);
     }
-    else {
-      if (key_addr \in malicious_virt_map) {
-        r <- is_key (oget phys_map.[oget malicious_virt_map.[key_addr]]);
-      }
-      else { r <- false; }
-    }
+    else { r <- false; }
     return r;
   }
 
   proc create_cell(pty : party, key_addr : addr, b : bool) : addr option = {
     var r : addr option;
     var phys_addr, virt_addr : addr;
-    if (pty = Honest) {
-      if (key_addr \in honest_virt_map) {
-        match oget phys_map.[oget honest_virt_map.[key_addr]] with
-        | Key key => {
-            phys_addr <@
-              phys_alloc(Cell {|key = key; cont = b; locked = true|});
-            virt_addr <@ honest_virt_alloc(phys_addr);
-            r <- Some virt_addr;
-          }
-        | Cell _  => { r <- None; }
-        end;
-      }
-      else { r <- None; }
+    if (key_addr \in oget virt_map.[pty]) {
+      match oget phys_map.[oget (oget virt_map.[pty]).[key_addr]] with
+      | Key key => {
+          phys_addr <@
+            phys_alloc(Cell {|key = key; cont = b; locked = true|});
+          virt_addr <@ virt_alloc(pty, phys_addr);
+          r <- Some virt_addr;
+        }
+      | Cell _  => { r <- None; }
+      end;
     }
-    else {
-      if (key_addr \in malicious_virt_map) {
-        match oget phys_map.[oget malicious_virt_map.[key_addr]] with
-        | Key key => {
-            phys_addr <@
-              phys_alloc(Cell {|key = key; cont = b; locked = true|});
-            virt_addr <@ malicious_virt_alloc(phys_addr);
-            r <- Some virt_addr;
-          }
-        | Cell _  => { r <- None; }
-        end;
-      }
-      else { r <- None; }
-    }
+    else { r <- None; }
     return r;
   }
 
   proc is_cell(pty : party, cell_addr : addr) : bool = {
     var r : bool;
-    if (pty = Honest) {
-      if (cell_addr \in honest_virt_map) {
-        r <- is_cell (oget phys_map.[oget honest_virt_map.[cell_addr]]);
-      }
-      else { r <- false; }
+    if (cell_addr \in oget virt_map.[pty]) {
+      r <- is_cell (oget phys_map.[oget (oget virt_map.[pty]).[cell_addr]]);
     }
-    else {
-      if (cell_addr \in malicious_virt_map) {
-        r <- is_cell (oget phys_map.[oget malicious_virt_map.[cell_addr]]);
-      }
-      else { r <- false; }
-    }
+    else { r <- false; }
     return r;
   }
 
   proc unlock_cell(pty : party, cell_addr : addr, key_addr : addr)
          : addr option = {
-    var r : addr option;
-    var phys_addr, virt_addr : addr;
-    var obj_cell, obj_key : object;
-    var cell : cell; var key : key;
-    if (pty = Honest) {
-      if (cell_addr \in honest_virt_map /\
-          key_addr  \in honest_virt_map) {
-        obj_cell <- oget phys_map.[oget honest_virt_map.[cell_addr]];
-        obj_key  <- oget phys_map.[oget honest_virt_map.[key_addr]];
-        if (is_cell obj_cell /\ is_key obj_key) {
-          cell <- oget (get_as_Cell obj_cell);
-          key  <- oget (get_as_Key obj_key);
-          if (cell.`key = key) {
-            cell <- {|cell with locked = false|};
-            phys_addr <@ phys_alloc(Cell cell);
-            virt_addr <@ honest_virt_alloc(phys_addr);
-            r <- Some virt_addr;
-          }
-          else { r <- None; }
+    var r : addr option; var phys_addr, virt_addr : addr;
+    var obj_cell, obj_key : object; var cell : cell; var key : key;
+    if (cell_addr \in oget virt_map.[pty] /\
+        key_addr  \in oget virt_map.[pty]) {
+      obj_cell <- oget phys_map.[oget (oget virt_map.[pty]).[cell_addr]];
+      obj_key  <- oget phys_map.[oget (oget virt_map.[pty]).[key_addr]];
+      if (is_cell obj_cell /\ is_key obj_key) {
+        cell <- oget (get_as_Cell obj_cell);
+        key  <- oget (get_as_Key obj_key);
+        if (cell.`key = key) {
+          cell <- {|cell with locked = false|};
+          phys_addr <@ phys_alloc(Cell cell);
+          virt_addr <@ virt_alloc(pty, phys_addr);
+          r <- Some virt_addr;
         }
         else { r <- None; }
       }
       else { r <- None; }
     }
-    else {
-      if (cell_addr \in malicious_virt_map /\
-          key_addr  \in malicious_virt_map) {
-        obj_cell <- oget phys_map.[oget malicious_virt_map.[cell_addr]];
-        obj_key  <- oget phys_map.[oget malicious_virt_map.[key_addr]];
-        if (is_cell obj_cell /\ is_key obj_key) {
-          cell <- oget (get_as_Cell obj_cell);
-          key  <- oget (get_as_Key obj_key);
-          if (cell.`key = key) {
-            cell <- {|cell with locked = false|};
-            phys_addr <@ phys_alloc(Cell cell);
-            virt_addr <@ malicious_virt_alloc(phys_addr);
-            r <- Some virt_addr;
-          }
-          else { r <- None; }
-        }
-        else { r <- None; }
-      }
-      else { r <- None; }
-    }
+    else { r <- None; }
     return r;
   }
 
   proc contents_cell(pty : party, cell_addr : addr) : bool option = {
     var r : bool option;
-    if (pty = Honest) {
-      if (cell_addr \in honest_virt_map) {
-        match oget phys_map.[oget honest_virt_map.[cell_addr]] with
-        | Key _     => { r <- None; }
-        | Cell cell => {
-            if (! cell.`locked) { r <- Some cell.`cont; }
-            else { r <- None; }
-          }
-        end;
-      }
-      else { r <- None; }
+    if (cell_addr \in oget virt_map.[pty]) {
+      match oget phys_map.[oget (oget virt_map.[pty]).[cell_addr]] with
+      | Key _     => { r <- None; }
+      | Cell cell => {
+          if (! cell.`locked) { r <- Some cell.`cont; }
+          else { r <- None; }
+        }
+      end;
     }
-    else {
-      if (cell_addr \in malicious_virt_map) {
-        match oget phys_map.[oget malicious_virt_map.[cell_addr]] with
-        | Key _     => { r <- None; }
-        | Cell cell => {
-            if (! cell.`locked) { r <- Some cell.`cont; }
-            else { r <- None; }
-          }
-        end;
-      }
-      else { r <- None; }
-    }
+    else { r <- None; }
     return r;
   }
 }.
@@ -384,46 +285,38 @@ module Memory : MEMORY = {
 
 type gm = glob Memory.
 
-op gm_to_next_key                 (gm : gm)  : key                 = gm.`5.
-op gm_to_next_phys_addr           (gm : gm)  : addr                = gm.`6.
-op gm_to_phys_map                 (gm : gm)  : (addr, object) fmap = gm.`7.
-op gm_to_honest_next_virt_addr    (gm : gm)  : addr                = gm.`1.
-op gm_to_honest_virt_map          (gm : gm)  : (addr, addr) fmap   = gm.`2.
-op gm_to_malicious_next_virt_addr (gm : gm)  : addr                = gm.`3.
-op gm_to_malicious_virt_map       (gm : gm)  : (addr, addr) fmap   = gm.`4.
+op gm_to_next_key       (gm : gm)  : key                             = gm.`1.
+op gm_to_next_phys_addr (gm : gm)  : addr                            = gm.`2.
+op gm_to_phys_map       (gm : gm)  : (addr, object) fmap             = gm.`4.
+op gm_to_next_virt_addr (gm : gm)  : (party, addr) fmap              = gm.`3.
+op gm_to_virt_map       (gm : gm)  : (party, (addr, addr) fmap) fmap = gm.`5.
 
 lemma gm_eqP (gm1 gm2 : gm) :
   gm_to_next_key gm1 = gm_to_next_key gm2 =>
   gm_to_next_phys_addr gm1 = gm_to_next_phys_addr gm2 =>
   gm_to_phys_map gm1 = gm_to_phys_map gm2 =>
-  gm_to_honest_next_virt_addr gm1 = gm_to_honest_next_virt_addr gm2 =>
-  gm_to_honest_virt_map gm1 = gm_to_honest_virt_map gm2 =>
-  gm_to_malicious_next_virt_addr gm1 = gm_to_malicious_next_virt_addr gm2 =>
-  gm_to_malicious_virt_map gm1 = gm_to_malicious_virt_map gm2 =>
+  gm_to_next_virt_addr gm1 = gm_to_next_virt_addr gm2 =>
+  gm_to_virt_map gm1 = gm_to_virt_map gm2 =>
   gm1 = gm2.
 proof. smt(). qed.
 
 (* invariant respected by the procedures of Memory *)
 
 op gm_invar_pre (gm : gm) : bool =
+  (forall (pty : party), pty \in gm_to_next_virt_addr gm) /\
+  (forall (pty : party), pty \in gm_to_virt_map gm) /\
   0 <= gm_to_next_key gm /\
   0 <= gm_to_next_phys_addr gm /\
-  0 <= gm_to_honest_next_virt_addr gm /\
-  0 <= gm_to_malicious_next_virt_addr gm /\
+  (forall (pty : party),
+   0 <= oget (gm_to_next_virt_addr gm).[pty]) /\
   (forall (addr : addr),
    addr \in gm_to_phys_map gm =>
    0 <= addr < gm_to_next_phys_addr gm) /\
-  (forall (addr : addr),
-   addr \in gm_to_honest_virt_map gm =>
-   0 <= addr < gm_to_honest_next_virt_addr gm) /\
-  (forall (addr : addr),
-   addr \in gm_to_malicious_virt_map gm =>
-   0 <= addr < gm_to_malicious_next_virt_addr gm) /\
-  (forall (addr : addr),
-   rng (gm_to_honest_virt_map gm) addr =>
-   addr \in gm_to_phys_map gm) /\
-  (forall (addr : addr),
-   rng (gm_to_malicious_virt_map gm) addr =>
+  (forall (pty : party, addr : addr),
+   addr \in oget (gm_to_virt_map gm).[pty] =>
+   0 <= addr < oget (gm_to_next_virt_addr gm).[pty]) /\
+  (forall (pty : party, addr : addr),
+   rng (oget (gm_to_virt_map gm).[pty]) addr =>
    addr \in gm_to_phys_map gm) /\
   (forall (addr1 addr2 : addr, key : key),
    (gm_to_phys_map gm).[addr1] = Some (Key key) =>
@@ -440,21 +333,21 @@ op gm_invar (gm : gm) : bool =
    (gm_to_phys_map gm).[addr] = Some (Key key) =>
    0 <= key < gm_to_next_key gm).
 
-lemma gm_invar_old_mal_virt_addr_does_not_give_new_key
-      (gm : gm, mal_virt_addr : addr) :
-  gm_invar gm => mal_virt_addr \in gm_to_malicious_virt_map gm =>
+lemma gm_invar_old_virt_addr_does_not_give_new_key
+      (gm : gm, pty : party, virt_addr : addr) :
+  gm_invar gm => virt_addr \in oget (gm_to_virt_map gm).[pty] =>
   let key = gm_to_next_key gm in
-  let phys_addr = oget (gm_to_malicious_virt_map gm).[mal_virt_addr] in
+  let phys_addr = oget (oget (gm_to_virt_map gm).[pty]).[virt_addr] in
   oget (gm_to_phys_map gm).[gm_to_next_phys_addr gm <- Key key].[phys_addr] <>
   Key key.
 proof.
-move => gm_invar_gm mal_virt_addr_in_dom_malicious_virt_map_of_gm /=.
+move => gm_invar_gm virt_addr_in_dom_virt_map_of_gm /=.
 have H1 :
-  oget (gm_to_malicious_virt_map gm).[mal_virt_addr] \in
-  gm_to_phys_map gm by smt().
+  oget (oget (gm_to_virt_map gm).[pty]).[virt_addr] \in
+  gm_to_phys_map gm by smt(get_some).
 have H2 :
-  oget (gm_to_malicious_virt_map gm).[mal_virt_addr] <>
-  gm_to_next_phys_addr gm by smt().
+  oget (oget (gm_to_virt_map gm).[pty]).[virt_addr] <>
+  gm_to_next_phys_addr gm by smt(get_some).
 rewrite get_setE H2 /= /#.
 qed.
 
@@ -470,16 +363,14 @@ lemma memory_init :
   hoare
   [Memory.init :
    true ==>
-   gm_invar (glob Memory)                  /\
-   Memory.next_key                 = 0     /\
-   Memory.next_phys_addr           = 0     /\
-   Memory.phys_map                 = empty /\
-   Memory.honest_next_virt_addr    = 0     /\
-   Memory.honest_virt_map          = empty /\
-   Memory.malicious_next_virt_addr = 0     /\
-   Memory.malicious_virt_map       = empty].
+   gm_invar (glob Memory) /\
+   Memory.next_key       = 0 /\
+   Memory.next_phys_addr = 0 /\
+   Memory.phys_map       = empty /\
+   Memory.next_virt_addr = empty.[Honest <- 0].[Malicious <- 0] /\
+   Memory.virt_map       = empty.[Honest <- empty].[Malicious <- empty]].
 proof.
-proc; auto; smt(mem_empty mem_rng_empty).
+proc; auto; smt(mem_set mem_empty mem_rng_empty get_setE get_some).
 qed.
 
 lemma memory_phys_alloc_key (gm : gm, key : key) :
@@ -493,16 +384,14 @@ lemma memory_phys_alloc_key (gm : gm, key : key) :
    gm_invar (glob Memory) /\
    (* unchanged *)
    Memory.next_key = gm_to_next_key gm /\
-   Memory.honest_next_virt_addr = gm_to_honest_next_virt_addr gm /\
-   Memory.honest_virt_map = gm_to_honest_virt_map gm /\
-   Memory.malicious_next_virt_addr = gm_to_malicious_next_virt_addr gm /\
-   Memory.malicious_virt_map = gm_to_malicious_virt_map gm /\
+   Memory.next_virt_addr = gm_to_next_virt_addr gm /\
+   Memory.virt_map = gm_to_virt_map gm /\
    (* changed *)
    Memory.next_phys_addr = gm_to_next_phys_addr gm + 1 /\
    Memory.phys_map = (gm_to_phys_map gm).[gm_to_next_phys_addr gm <- Key key] /\
    res = gm_to_next_phys_addr gm].
 proof.
-proc; auto; smt(get_setE).
+proc; auto; progress; smt(get_setE).
 qed.
 
 lemma memory_phys_alloc_cell (gm : gm, cell : cell) :
@@ -514,59 +403,37 @@ lemma memory_phys_alloc_cell (gm : gm, cell : cell) :
    gm_invar (glob Memory) /\
    (* unchanged *)
    Memory.next_key = gm_to_next_key gm /\
-   Memory.honest_next_virt_addr = gm_to_honest_next_virt_addr gm /\
-   Memory.honest_virt_map = gm_to_honest_virt_map gm /\
-   Memory.malicious_next_virt_addr = gm_to_malicious_next_virt_addr gm /\
-   Memory.malicious_virt_map = gm_to_malicious_virt_map gm /\
+   Memory.next_virt_addr = gm_to_next_virt_addr gm /\
+   Memory.virt_map = gm_to_virt_map gm /\
    (* changed *)
    Memory.next_phys_addr = gm_to_next_phys_addr gm + 1 /\
    Memory.phys_map = (gm_to_phys_map gm).[gm_to_next_phys_addr gm <- Cell cell] /\
    res = gm_to_next_phys_addr gm].
 proof.
-proc; auto; smt(get_setE).
+proc; auto; progress; smt(get_setE).
 qed.
 
-lemma memory_honest_virt_alloc (gm : gm, phys_addr' : addr) :
+lemma memory_virt_alloc (gm : gm, pty' : party, phys_addr' : addr) :
   hoare
-  [Memory.honest_virt_alloc :
-   phys_addr = phys_addr' /\ phys_addr' \in Memory.phys_map /\
+  [Memory.virt_alloc :
+   pty = pty' /\ phys_addr = phys_addr' /\ phys_addr' \in Memory.phys_map /\
    glob Memory = gm /\ gm_invar gm ==>
    gm_invar (glob Memory) /\
    (* unchanged *)
    Memory.next_key = gm_to_next_key gm /\
    Memory.next_phys_addr = gm_to_next_phys_addr gm /\
    Memory.phys_map = gm_to_phys_map gm /\
-   Memory.malicious_next_virt_addr = gm_to_malicious_next_virt_addr gm /\
-   Memory.malicious_virt_map = gm_to_malicious_virt_map gm /\
+   Memory.next_virt_addr.[other pty'] = (gm_to_next_virt_addr gm).[other pty'] /\
+   Memory.virt_map.[other pty'] = (gm_to_virt_map gm).[other pty'] /\
    (* changed *)
-   Memory.honest_next_virt_addr = gm_to_honest_next_virt_addr gm + 1 /\
-   Memory.honest_virt_map =
-   (gm_to_honest_virt_map gm).[gm_to_honest_next_virt_addr gm <- phys_addr'] /\
-   res = gm_to_honest_next_virt_addr gm].
+   oget Memory.next_virt_addr.[pty'] =
+     oget (gm_to_next_virt_addr gm).[pty'] + 1 /\
+   oget Memory.virt_map.[pty'] =
+   (oget (gm_to_virt_map gm).[pty'])
+     .[oget (gm_to_next_virt_addr gm).[pty'] <- phys_addr'] /\
+   res = oget (gm_to_next_virt_addr gm).[pty']].
 proof.
-proc; auto; smt(mem_set rng_set_new).
-qed.
-
-lemma memory_malicious_virt_alloc (gm : gm, phys_addr' : addr) :
-  hoare
-  [Memory.malicious_virt_alloc :
-   phys_addr = phys_addr' /\ phys_addr' \in Memory.phys_map /\
-   glob Memory = gm /\ gm_invar gm ==>
-   gm_invar (glob Memory) /\
-   (* unchanged *)
-   Memory.next_key = gm_to_next_key gm /\
-   Memory.next_phys_addr = gm_to_next_phys_addr gm /\
-   Memory.phys_map = gm_to_phys_map gm /\
-   Memory.honest_next_virt_addr = gm_to_honest_next_virt_addr gm /\
-   Memory.honest_virt_map = gm_to_honest_virt_map gm /\
-   (* changed *)
-   Memory.malicious_next_virt_addr = gm_to_malicious_next_virt_addr gm + 1 /\
-   Memory.malicious_virt_map =
-   (gm_to_malicious_virt_map gm).[gm_to_malicious_next_virt_addr gm <-
-                                  phys_addr'] /\
-   res = gm_to_malicious_next_virt_addr gm].
-proof.
-proc; auto; smt(mem_set rng_set_new).
+proc; auto; smt(mem_set rng_set_new get_some get_setE).
 qed.
 
 lemma memory_trans_virt_addr_ll :
@@ -578,69 +445,51 @@ lemma memory_trans_virt_addr_gm_invar :
   [Memory.trans_virt_addr :
    gm_invar (glob Memory) ==> gm_invar (glob Memory)].
 proof.
-proc; inline*; auto; smt(mem_set rng_set_new).
+proc; inline*; auto.
+(progress; first 8 smt(get_setE get_some)); last 5 smt(get_setE get_some).
+rewrite /gm_to_next_virt_addr /=; smt(get_setE get_some).
 qed.
 
 lemma memory_trans_virt_addr (gm : gm, pty' : party, addr' : addr) :
   hoare
   [Memory.trans_virt_addr :
    pty = pty' /\ addr = addr' /\
-   (if pty = Honest
-    then addr \in Memory.honest_virt_map
-    else addr \in Memory.malicious_virt_map) /\
+   addr \in oget Memory.virt_map.[pty] /\
    glob Memory = gm /\ gm_invar gm ==>
    gm_invar (glob Memory) /\
    (* unchanged *)
    Memory.next_key = gm_to_next_key gm /\
    Memory.next_phys_addr = gm_to_next_phys_addr gm /\
    Memory.phys_map = gm_to_phys_map gm /\
+   Memory.next_virt_addr.[pty'] = (gm_to_next_virt_addr gm).[pty'] /\
+   Memory.virt_map.[pty'] = (gm_to_virt_map gm).[pty'] /\
    (* changed *)
-   if pty' = Honest
-   then (let phys_addr = oget (Memory.honest_virt_map.[addr']) in
-         let virt_addr_malic = gm_to_malicious_next_virt_addr gm in
-         Memory.honest_next_virt_addr = gm_to_honest_next_virt_addr gm /\
-         Memory.honest_virt_map = gm_to_honest_virt_map gm /\
-         Memory.malicious_next_virt_addr = virt_addr_malic + 1 /\
-         Memory.malicious_virt_map =
-         (gm_to_malicious_virt_map gm).[virt_addr_malic <- phys_addr] /\
-         res = Some virt_addr_malic)
-   else (let phys_addr = oget (Memory.malicious_virt_map.[addr']) in
-         let virt_addr_honest = gm_to_honest_next_virt_addr gm in
-         Memory.malicious_next_virt_addr = gm_to_malicious_next_virt_addr gm /\
-         Memory.malicious_virt_map = gm_to_malicious_virt_map gm /\
-         Memory.honest_next_virt_addr = virt_addr_honest + 1 /\
-         Memory.honest_virt_map =
-         (gm_to_honest_virt_map gm).[virt_addr_honest <- phys_addr] /\
-         res = Some virt_addr_honest)].
+   let phys_addr = oget (oget (Memory.virt_map.[pty'])).[addr'] in
+   let next_virt_addr_other = oget (gm_to_next_virt_addr gm).[other pty'] in
+   oget Memory.next_virt_addr.[other pty'] =
+     next_virt_addr_other + 1 /\
+   oget Memory.virt_map.[other pty'] =
+   (oget (gm_to_virt_map gm).[other pty'])
+     .[next_virt_addr_other <- phys_addr] /\
+   res = Some next_virt_addr_other].
 proof.
 proc.
 if.
-rcondt 1; first auto.
-sp.
-exlim phys_addr => pa'.
-exlim (glob Memory) => gm'.
-wp.
-call (memory_malicious_virt_alloc gm' pa').
-auto; smt().
-rcondt 1; first auto; smt().
-sp.
-exlim phys_addr => pa'.
-exlim (glob Memory) => gm'.
-wp.
-call (memory_honest_virt_alloc gm' pa').
+sp; wp.
+exlim (glob Memory), phys_addr => gm' pa'.
+call (memory_virt_alloc gm' (other pty') pa').
+auto; smt(get_setE get_some).
 auto; smt().
 qed.
 
 lemma memory_trans_virt_addr_bad (gm : gm) :
   hoare
   [Memory.trans_virt_addr :
-   (if pty = Honest
-    then addr \notin Memory.honest_virt_map
-    else addr \notin Memory.malicious_virt_map) /\
+   addr \notin oget Memory.virt_map.[pty] /\
    glob Memory = gm /\ gm_invar gm ==>
    glob Memory = gm /\ gm_invar (glob Memory)].
 proof.
-proc; if; [rcondf 1; auto | rcondf 1; auto; smt()].
+proc; inline*; if; auto.
 qed.
 
 lemma memory_create_key_ll : islossless Memory.create_key.
@@ -664,23 +513,15 @@ lemma memory_create_key (gm : gm, pty' : party) :
    Memory.phys_map =
    (gm_to_phys_map gm)
      .[gm_to_next_phys_addr gm <- Key (gm_to_next_key gm)] /\
-   (if pty' = Honest
-    then (Memory.honest_next_virt_addr =
-          gm_to_honest_next_virt_addr gm + 1 /\
-          Memory.honest_virt_map =
-          (gm_to_honest_virt_map gm)
-            .[gm_to_honest_next_virt_addr gm <- gm_to_next_phys_addr gm] /\
-          res = gm_to_honest_next_virt_addr gm /\
-          Memory.malicious_next_virt_addr = gm_to_malicious_next_virt_addr gm /\
-          Memory.malicious_virt_map = gm_to_malicious_virt_map gm)
-    else (Memory.malicious_next_virt_addr =
-          gm_to_malicious_next_virt_addr gm + 1 /\
-          Memory.malicious_virt_map =
-          (gm_to_malicious_virt_map gm)
-            .[gm_to_malicious_next_virt_addr gm <- gm_to_next_phys_addr gm] /\
-          res = gm_to_malicious_next_virt_addr gm /\
-          Memory.honest_next_virt_addr = gm_to_honest_next_virt_addr gm /\
-          Memory.honest_virt_map = gm_to_honest_virt_map gm))].
+   oget Memory.next_virt_addr.[pty'] =
+   oget (gm_to_next_virt_addr gm).[pty'] + 1 /\
+   oget Memory.virt_map.[pty'] =
+   (oget (gm_to_virt_map gm).[pty'])
+     .[oget (gm_to_next_virt_addr gm).[pty'] <-
+       gm_to_next_phys_addr gm] /\
+   Memory.next_virt_addr.[other pty'] = (gm_to_next_virt_addr gm).[other pty'] /\
+   Memory.virt_map.[other pty'] = (gm_to_virt_map gm).[other pty'] /\
+   res = oget (gm_to_next_virt_addr gm).[pty']].
 proof.
 proc.
 sp.
@@ -691,51 +532,31 @@ seq 1 :
    Memory.next_phys_addr = gm_to_next_phys_addr gm + 1 /\
    Memory.phys_map =
    (gm_to_phys_map gm).[gm_to_next_phys_addr gm <- Key key] /\
-   Memory.honest_next_virt_addr = gm_to_honest_next_virt_addr gm /\
-   Memory.honest_virt_map = gm_to_honest_virt_map gm /\
-   Memory.malicious_next_virt_addr = gm_to_malicious_next_virt_addr gm /\
-   Memory.malicious_virt_map = gm_to_malicious_virt_map gm) => //.
-auto.
+   Memory.next_virt_addr = gm_to_next_virt_addr gm /\
+   Memory.virt_map = gm_to_virt_map gm).
 exlim (glob Memory) => gm'.
 exlim key => key'.
 call (memory_phys_alloc_key gm' key').
 auto; smt().
-if.
 exlim (glob Memory) => gm'.
 exlim phys_addr => phys_addr'.
-call (memory_honest_virt_alloc gm' phys_addr').
-auto; progress; smt(mem_set get_setE).
-exlim (glob Memory) => gm'.
-exlim phys_addr => phys_addr'.
-call (memory_malicious_virt_alloc gm' phys_addr').
-auto; progress; smt(mem_set get_setE).
+call (memory_virt_alloc gm' pty' phys_addr').
+auto; smt(mem_set get_setE).
 qed.
 
 op key_addr_good (pty : party, gm : gm, key_addr : addr) : bool =
-  if pty = Honest
-  then (key_addr \in (gm_to_honest_virt_map gm) /\
-        is_key
-        (oget
-         ((gm_to_phys_map gm)
-            .[oget ((gm_to_honest_virt_map gm).[key_addr])])))
-  else (key_addr \in (gm_to_malicious_virt_map gm) /\
-        is_key
-        (oget
-         ((gm_to_phys_map gm)
-            .[oget ((gm_to_malicious_virt_map gm).[key_addr])]))).
+  key_addr \in oget (gm_to_virt_map gm).[pty] /\
+  is_key
+  (oget
+   ((gm_to_phys_map gm)
+      .[oget (oget (gm_to_virt_map gm).[pty]).[key_addr]])).
 
 op key_addr_to_key (pty : party, gm : gm, key_addr : addr) : key =
-  if pty = Honest
-  then oget
-       (get_as_Key
-        (oget
-         ((gm_to_phys_map gm)
-            .[oget ((gm_to_honest_virt_map gm).[key_addr])])))
-  else oget
-       (get_as_Key
-        (oget
-         ((gm_to_phys_map gm)
-            .[oget ((gm_to_malicious_virt_map gm).[key_addr])]))).
+  oget
+  (get_as_Key
+   (oget
+    ((gm_to_phys_map gm)
+       .[oget (oget (gm_to_virt_map gm).[pty]).[key_addr]]))).
 
 lemma memory_is_key_ll : islossless Memory.is_key.
 proof. islossless. qed.
@@ -769,7 +590,6 @@ lemma memory_create_cell_ll : islossless Memory.create_cell.
 proof.
 islossless.
 match; islossless.
-match; islossless.
 qed.
 
 lemma memory_create_cell_gm_invar :
@@ -777,13 +597,15 @@ lemma memory_create_cell_gm_invar :
   [Memory.create_cell :
    gm_invar (glob Memory) ==> gm_invar (glob Memory)].
 proof.
-proc; if; if.
+proc; if.
 match.
-inline*; auto; progress; smt(mem_set get_setE).
-auto.
-auto.
-match.
-inline*; auto; progress; smt(mem_set get_setE).
+(inline*; auto; progress; first 11 smt(mem_set get_setE oget_some));
+  last 2 smt(get_setE oget_some).
+move : H2; rewrite /gm_to_phys_map /= get_setE.
+case (addr = Memory.next_phys_addr{hr}) => /= [addr_eq_npa <- | addr_ne_npa].
+exists (oget (oget Memory.virt_map{hr}.[pty{hr}]).[key_addr{hr}]).
+smt(get_setE oget_some some_oget).
+smt(get_setE oget_some some_oget).
 auto.
 auto.
 qed.
@@ -797,43 +619,29 @@ lemma memory_create_cell
    gm_invar (glob Memory) /\
    Memory.next_key = gm_to_next_key gm /\
    Memory.next_phys_addr = gm_to_next_phys_addr gm + 1 /\
-   (if pty' = Honest
-    then (let key = key_addr_to_key Honest gm key_addr' in
-          Memory.phys_map =
-          (gm_to_phys_map gm)
-             .[gm_to_next_phys_addr gm <-
-               Cell {|key = key; cont = b'; locked = true|}] /\
-          Memory.honest_next_virt_addr =
-          gm_to_honest_next_virt_addr gm + 1 /\
-          Memory.honest_virt_map =
-          (gm_to_honest_virt_map gm)
-             .[gm_to_honest_next_virt_addr gm <- gm_to_next_phys_addr gm] /\
-          res = Some (gm_to_honest_next_virt_addr gm) /\
-          Memory.malicious_next_virt_addr = gm_to_malicious_next_virt_addr gm /\
-          Memory.malicious_virt_map = gm_to_malicious_virt_map gm)
-    else (let key = key_addr_to_key Malicious gm key_addr' in
-          Memory.phys_map =
-          (gm_to_phys_map gm)
-             .[gm_to_next_phys_addr gm <-
-               Cell {|key = key; cont = b'; locked = true|}] /\
-          Memory.malicious_next_virt_addr =
-          gm_to_malicious_next_virt_addr gm + 1 /\
-          Memory.malicious_virt_map =
-          (gm_to_malicious_virt_map gm)
-             .[gm_to_malicious_next_virt_addr gm <- gm_to_next_phys_addr gm] /\
-          res = Some (gm_to_malicious_next_virt_addr gm) /\
-          Memory.honest_next_virt_addr = gm_to_honest_next_virt_addr gm /\
-          Memory.honest_virt_map = gm_to_honest_virt_map gm))].
+   Memory.phys_map =
+   (gm_to_phys_map gm)
+      .[gm_to_next_phys_addr gm <-
+        Cell
+        {|key = key_addr_to_key pty' gm key_addr';
+          cont = b'; locked = true|}] /\
+   oget Memory.next_virt_addr.[pty'] =
+   oget (gm_to_next_virt_addr gm).[pty'] + 1 /\
+   oget Memory.virt_map.[pty'] =
+   (oget (gm_to_virt_map gm).[pty'])
+      .[oget (gm_to_next_virt_addr gm).[pty'] <- gm_to_next_phys_addr gm] /\
+   Memory.next_virt_addr.[other pty'] = (gm_to_next_virt_addr gm).[other pty'] /\
+   Memory.virt_map.[other pty'] = (gm_to_virt_map gm).[other pty'] /\
+   res = Some (oget (gm_to_next_virt_addr gm).[pty'])].
 proof.
-proc.
-if.
+proc => /=.
 rcondt 1; first auto; smt().
 match Key 1; first auto; smt().
 exlim key => key'.
 seq 1 :
-  (pty = pty' /\ pty' = Honest /\ key_addr' \in gm_to_honest_virt_map gm /\
-   key_addr_good Honest gm key_addr' /\
-   key' = key_addr_to_key Honest gm key_addr' /\
+  (pty = pty' /\ key_addr' \in oget (gm_to_virt_map gm).[pty'] /\
+   key_addr_good pty' gm key_addr' /\
+   key' = key_addr_to_key pty' gm key_addr' /\
    gm_invar gm /\ phys_addr = gm_to_next_phys_addr gm /\
    Memory.next_key = gm_to_next_key gm /\
    Memory.next_phys_addr = gm_to_next_phys_addr gm + 1 /\
@@ -841,42 +649,19 @@ seq 1 :
    (gm_to_phys_map gm)
      .[gm_to_next_phys_addr gm <-
        Cell {|key = key'; cont = b'; locked = true|}] /\
-   Memory.honest_next_virt_addr = gm_to_honest_next_virt_addr gm /\
-   Memory.honest_virt_map = gm_to_honest_virt_map gm /\
-   Memory.malicious_next_virt_addr = gm_to_malicious_next_virt_addr gm /\
-   Memory.malicious_virt_map = gm_to_malicious_virt_map gm) => //.
+   Memory.next_virt_addr = gm_to_next_virt_addr gm /\
+   Memory.virt_map = gm_to_virt_map gm).
 call (memory_phys_alloc_cell gm {|key = key'; cont = b'; locked = true|}).
-auto; progress; smt().
+auto; progress [-delta];
+  have /# :
+    Memory.phys_map{hr}
+      .[oget (oget Memory.virt_map{hr}.[pty{hr}]).[key_addr{hr}]] =
+    Some (Key key{hr}) by smt(get_some).
 wp.
 exlim (glob Memory) => gm'.
 exlim phys_addr => phys_addr'.
-call (memory_honest_virt_alloc gm' phys_addr').
+call (memory_virt_alloc gm' pty' phys_addr').
 auto => /> /= ; progress; smt(mem_set get_setE).
-rcondt 1; first auto; smt().
-match Key 1; first auto; smt().
-exlim key => key'.
-seq 1 :
-  (pty = pty' /\ pty' = Malicious /\ key_addr' \in gm_to_malicious_virt_map gm /\
-   key_addr_good Malicious gm key_addr' /\
-   key' = key_addr_to_key Malicious gm key_addr' /\
-   gm_invar gm /\ phys_addr = gm_to_next_phys_addr gm /\
-   Memory.next_key = gm_to_next_key gm /\
-   Memory.next_phys_addr = gm_to_next_phys_addr gm + 1 /\
-   Memory.phys_map =
-   (gm_to_phys_map gm)
-     .[gm_to_next_phys_addr gm <-
-       Cell {|key = key'; cont = b'; locked = true|}] /\
-   Memory.malicious_next_virt_addr = gm_to_malicious_next_virt_addr gm /\
-   Memory.malicious_virt_map = gm_to_malicious_virt_map gm /\
-   Memory.honest_next_virt_addr = gm_to_honest_next_virt_addr gm /\
-   Memory.honest_virt_map = gm_to_honest_virt_map gm) => //.
-call (memory_phys_alloc_cell gm {|key = key'; cont = b'; locked = true|}).
-auto; progress; smt().
-wp.
-exlim (glob Memory) => gm'.
-exlim phys_addr => phys_addr'.
-call (memory_malicious_virt_alloc gm' phys_addr').
-auto => /> /=; progress; smt(mem_set get_setE).
 qed.
 
 lemma memory_create_cell_bad (gm : gm) :
@@ -888,40 +673,28 @@ lemma memory_create_cell_bad (gm : gm) :
    Memory.next_key = gm_to_next_key gm /\
    Memory.next_phys_addr = gm_to_next_phys_addr gm /\
    Memory.phys_map = gm_to_phys_map gm /\
-   Memory.honest_next_virt_addr = gm_to_honest_next_virt_addr gm /\
-   Memory.honest_virt_map = gm_to_honest_virt_map gm /\
-   Memory.malicious_next_virt_addr = gm_to_malicious_next_virt_addr gm /\
-   Memory.malicious_virt_map = gm_to_malicious_virt_map gm /\
+   Memory.next_virt_addr = gm_to_next_virt_addr gm /\
+   Memory.virt_map = gm_to_virt_map gm /\
    res = None].
 proof.
-proc; if; (if; [match Cell 1; [auto; smt() | auto] | auto]).
+proc => /=; if.
+match Cell 1; auto; smt().
+auto.
 qed.
 
 op cell_addr_good (pty : party, gm : gm, cell_addr : addr) : bool =
-  if pty = Honest
-  then (cell_addr \in (gm_to_honest_virt_map gm) /\
-        is_cell
-        (oget
-         ((gm_to_phys_map gm)
-            .[oget ((gm_to_honest_virt_map gm).[cell_addr])])))
-  else (cell_addr \in (gm_to_malicious_virt_map gm) /\
-        is_cell
-        (oget
-         ((gm_to_phys_map gm)
-            .[oget ((gm_to_malicious_virt_map gm).[cell_addr])]))).
+  cell_addr \in oget (gm_to_virt_map gm).[pty] /\
+  is_cell
+  (oget
+   ((gm_to_phys_map gm)
+      .[oget (oget (gm_to_virt_map gm).[pty]).[cell_addr]])).
 
 op cell_addr_to_cell (pty : party, gm : gm, cell_addr : addr) : cell =
-  if pty = Honest
-  then oget
-       (get_as_Cell
-        (oget
-         ((gm_to_phys_map gm)
-            .[oget ((gm_to_honest_virt_map gm).[cell_addr])])))
-  else oget
-       (get_as_Cell
-        (oget
-         ((gm_to_phys_map gm)
-            .[oget ((gm_to_malicious_virt_map gm).[cell_addr])]))).
+  oget
+  (get_as_Cell
+   (oget
+    ((gm_to_phys_map gm)
+       .[oget (oget (gm_to_virt_map gm).[pty]).[cell_addr]]))).
 
 lemma good_cell_addr_key_in_mem (pty : party, gm : gm, cell_addr : addr) :
   gm_invar gm => cell_addr_good pty gm cell_addr =>
@@ -931,21 +704,17 @@ lemma good_cell_addr_key_in_mem (pty : party, gm : gm, cell_addr : addr) :
 proof.
 move => gmi_gm.
 rewrite /cell_addr_good /cell_addr_to_cell.
-case pty => /=.
 move => [H1 H2].
 have [cell H3] :
   exists cell,
-  oget (gm_to_phys_map gm)
-         .[oget (gm_to_honest_virt_map gm).[cell_addr]] =
+  oget
+  (gm_to_phys_map gm)
+    .[oget (oget (gm_to_virt_map gm).[pty]).[cell_addr]] =
   Cell cell by smt().
-rewrite /get_as_Cell H3 /= /#.
-move => [H1 H2].
-have [cell H3] :
-  exists cell,
-  oget (gm_to_phys_map gm)
-         .[oget (gm_to_malicious_virt_map gm).[cell_addr]] =
-  Cell cell by smt().
-rewrite /get_as_Cell H3 /= /#.
+rewrite /get_as_Cell H3 /=.
+have /# :
+  (gm_to_phys_map gm).[oget (oget (gm_to_virt_map gm).[pty]).[cell_addr]] =
+  Some (Cell cell) by smt(get_some).
 qed.
 
 op good_cell_addr_unlocked_by_good_key_addr
@@ -995,80 +764,12 @@ lemma memory_unlock_cell_gm_invar :
   [Memory.unlock_cell :
    gm_invar (glob Memory) ==> gm_invar (glob Memory)].
 proof.
-proc; if; if; sp.
-if.
-sp.
-if.
+proc; if; last auto.
+sp; if; last auto.
+sp; if; last auto.
 sp; wp; elim* => cell0; inline*.
-(auto; progress; first 4 smt()); first 6 smt(get_setE).
-smt(get_setE rng_set_new). smt(get_setE). smt(get_setE).
-rewrite /gm_to_phys_map /= in H5. rewrite /gm_to_phys_map /=.
-case (addr = Memory.next_phys_addr{hr}) => [eq_addr_npa | neq_addr_npa].
-move : H5.
-rewrite get_setE eq_addr_npa /=.
-move => <- /=.
-pose cell1 :=
-  oget
-  (get_as_Cell
-   (oget
-    Memory.phys_map{hr}
-      .[oget Memory.honest_virt_map{hr}.[cell_addr{hr}]])).
-have [addr'] eq_pm_addr'_cell1_key :
-  exists addr',
-  Memory.phys_map{hr}.[addr'] = Some (Key cell1.`key) by smt().
-exists addr'.
-have ne_addr'_npa : addr' <> Memory.next_phys_addr{hr} by smt(domE).
-by rewrite get_setE ne_addr'_npa /=.
-move : H5 => H5.
-rewrite get_setE neq_addr_npa /= in H5.
-have [addr' eq_pm_addr'_cell0_key] :
-  exists addr',
-  Memory.phys_map{hr}.[addr'] = Some (Key cell0.`key)
-    by smt().
-exists addr'.
-have neq_addr'_npa : addr' <> Memory.next_phys_addr{hr} by smt(domE).
-by rewrite get_setE neq_addr'_npa /=.
-smt(get_setE). smt(get_setE).
-auto.
-auto.
-auto.
-if.
-sp.
-if.
-sp; wp; elim* => cell0; inline*.
-(auto; progress; first 4 smt()); first 6 smt(get_setE).
-smt(get_setE rng_set_new). smt(mem_set get_setE).
-smt(get_setE).
-rewrite /gm_to_phys_map /= in H6. rewrite /gm_to_phys_map /=.
-case (addr = Memory.next_phys_addr{hr}) => [eq_addr_npa | neq_addr_npa].
-move : H6.
-rewrite get_setE eq_addr_npa /=.
-move => <- /=.
-pose cell1 :=
-  oget
-  (get_as_Cell
-   (oget
-    Memory.phys_map{hr}
-      .[oget Memory.malicious_virt_map{hr}.[cell_addr{hr}]])).
-have [addr'] eq_pm_addr'_cell1_key :
-  exists addr',
-  Memory.phys_map{hr}.[addr'] = Some (Key cell1.`key) by smt().
-exists addr'.
-have ne_addr'_npa : addr' <> Memory.next_phys_addr{hr} by smt(domE).
-by rewrite get_setE ne_addr'_npa /=.
-move : H6 => H6.
-rewrite get_setE neq_addr_npa /= in H6.
-have [addr' eq_pm_addr'_cell0_key] :
-  exists addr',
-  Memory.phys_map{hr}.[addr'] = Some (Key cell0.`key)
-    by smt().
-exists addr'.
-have neq_addr'_npa : addr' <> Memory.next_phys_addr{hr} by smt(domE).
-by rewrite get_setE neq_addr'_npa /=.
-smt(get_setE). smt(get_setE).
-auto.
-auto.
-auto.
+(auto; progress; first 7 smt(get_setE)); last 6 smt(oget_some get_setE).
+move : H5; rewrite /gm_to_virt_map /= get_setE /=; smt(mem_set).
 qed.
 
 lemma memory_unlock_cell (gm : gm , pty' : party, cell_addr' key_addr' : addr) :
@@ -1081,48 +782,33 @@ lemma memory_unlock_cell (gm : gm , pty' : party, cell_addr' key_addr' : addr) :
    gm_invar (glob Memory) /\
    Memory.next_key = gm_to_next_key gm /\
    Memory.next_phys_addr = gm_to_next_phys_addr gm + 1 /\
-   (if pty' = Honest
-    then (let cell = cell_addr_to_cell Honest gm cell_addr' in
-          Memory.phys_map =
-          (gm_to_phys_map gm)
-             .[gm_to_next_phys_addr gm <-
-               Cell {|cell with locked = false|}] /\
-          Memory.honest_next_virt_addr =
-          gm_to_honest_next_virt_addr gm + 1 /\
-          Memory.honest_virt_map =
-          (gm_to_honest_virt_map gm)
-             .[gm_to_honest_next_virt_addr gm <- gm_to_next_phys_addr gm] /\
-          res = Some (gm_to_honest_next_virt_addr gm) /\
-          Memory.malicious_next_virt_addr = gm_to_malicious_next_virt_addr gm /\
-          Memory.malicious_virt_map = gm_to_malicious_virt_map gm)
-    else (let cell = cell_addr_to_cell Malicious gm cell_addr' in
-          Memory.phys_map =
-          (gm_to_phys_map gm)
-             .[gm_to_next_phys_addr gm <-
-               Cell {|cell with locked = false|}] /\
-          Memory.malicious_next_virt_addr =
-          gm_to_malicious_next_virt_addr gm + 1 /\
-          Memory.malicious_virt_map =
-          (gm_to_malicious_virt_map gm)
-             .[gm_to_malicious_next_virt_addr gm <- gm_to_next_phys_addr gm] /\
-          res = Some (gm_to_malicious_next_virt_addr gm) /\
-          Memory.honest_next_virt_addr = gm_to_honest_next_virt_addr gm /\
-          Memory.honest_virt_map = gm_to_honest_virt_map gm))].
+   Memory.phys_map =
+   (gm_to_phys_map gm)
+     .[gm_to_next_phys_addr gm <-
+       Cell
+       {|(cell_addr_to_cell pty' gm cell_addr') with locked = false|}] /\
+   oget Memory.next_virt_addr.[pty'] =
+   oget (gm_to_next_virt_addr gm).[pty'] + 1 /\
+   oget Memory.virt_map.[pty'] =
+   (oget (gm_to_virt_map gm).[pty'])
+     .[oget (gm_to_next_virt_addr gm).[pty'] <- gm_to_next_phys_addr gm] /\
+   Memory.next_virt_addr.[other pty'] = 
+   (gm_to_next_virt_addr gm).[other pty'] /\
+   Memory.virt_map.[other pty'] =  (gm_to_virt_map gm).[other pty'] /\
+   res = Some (oget (gm_to_next_virt_addr gm).[pty'])].
 proof.
 proc.
-if.
 rcondt 1; first auto; smt().
 sp 2.
 rcondt 1; first auto; smt().
 sp 2.
 rcondt 1; first auto; smt().
 sp 1.
-elim* => cell'.
-rewrite /=.
+elim* => cell' /=.
 seq 1 :
-  (pty = pty' /\ pty' = Honest /\ gm_invar gm /\
+  (pty = pty' /\ gm_invar gm /\
    cell' = cell_addr_to_cell pty gm cell_addr' /\
-   cell_addr_good Honest gm cell_addr' /\
+   cell_addr_good pty gm cell_addr' /\
    phys_addr = gm_to_next_phys_addr gm /\
    Memory.next_key = gm_to_next_key gm /\
    Memory.next_phys_addr = gm_to_next_phys_addr gm + 1 /\
@@ -1130,46 +816,14 @@ seq 1 :
    (gm_to_phys_map gm)
      .[gm_to_next_phys_addr gm <-
        Cell {|cell' with locked = false|}] /\
-   Memory.honest_next_virt_addr = gm_to_honest_next_virt_addr gm /\
-   Memory.honest_virt_map = gm_to_honest_virt_map gm /\
-   Memory.malicious_next_virt_addr = gm_to_malicious_next_virt_addr gm /\
-   Memory.malicious_virt_map = gm_to_malicious_virt_map gm) => //.
+   Memory.next_virt_addr = gm_to_next_virt_addr gm /\
+   Memory.virt_map = gm_to_virt_map gm).
 call (memory_phys_alloc_cell gm {|cell' with locked = false|}).
 auto; smt().
 wp => /=.
 exlim (glob Memory) => gm'.
 exlim phys_addr => phys_addr'.
-call (memory_honest_virt_alloc gm' phys_addr').
-auto; progress; smt(mem_set rng_set_new get_setE good_cell_addr_key_in_mem).
-rcondt 1; first auto; smt().
-sp 2.
-rcondt 1; first auto; smt().
-sp 2.
-rcondt 1; first auto; smt().
-sp 1.
-elim* => cell'.
-rewrite /=.
-seq 1 :
-  (pty = pty' /\ pty' = Malicious /\ gm_invar gm /\
-   cell' = cell_addr_to_cell pty gm cell_addr' /\
-   cell_addr_good Malicious gm cell_addr' /\
-   phys_addr = gm_to_next_phys_addr gm /\
-   Memory.next_key = gm_to_next_key gm /\
-   Memory.next_phys_addr = gm_to_next_phys_addr gm + 1 /\
-   Memory.phys_map =
-   (gm_to_phys_map gm)
-     .[gm_to_next_phys_addr gm <-
-       Cell {|cell' with locked = false|}] /\
-   Memory.honest_next_virt_addr = gm_to_honest_next_virt_addr gm /\
-   Memory.honest_virt_map = gm_to_honest_virt_map gm /\
-   Memory.malicious_next_virt_addr = gm_to_malicious_next_virt_addr gm /\
-   Memory.malicious_virt_map = gm_to_malicious_virt_map gm) => //.
-call (memory_phys_alloc_cell gm {|cell' with locked = false|}).
-auto; progress; smt().
-wp => /=.
-exlim (glob Memory) => gm'.
-exlim phys_addr => phys_addr'.
-call (memory_malicious_virt_alloc gm' phys_addr').
+call (memory_virt_alloc gm' pty' phys_addr').
 auto; progress; smt(mem_set rng_set_new get_setE good_cell_addr_key_in_mem).
 qed.
 
@@ -1184,13 +838,12 @@ lemma memory_unlock_cell_bad
    glob Memory = gm /\ gm_invar (glob Memory) /\ res = None].
 proof.
 proc.
-if; (if; [sp; if; [sp; if; [exfalso; smt() | auto] | auto] | auto]).
+if; [sp; if; [sp; if; [exfalso; smt() | auto] | auto] | auto].
 qed.
 
 lemma memory_contents_cell_ll : islossless Memory.contents_cell.
 proof.
 islossless.
-match; islossless.
 match; islossless.
 qed.
 
@@ -1214,11 +867,6 @@ lemma memory_contents_cell (gm : gm , pty' : party, cell_addr' : addr) :
     res = Some cell.`cont)].
 proof.
 proc.
-if.
-rcondt 1; first auto; smt().
-match Cell 1; first auto; smt().
-rcondt 1; first auto; smt().
-auto; smt().
 rcondt 1; first auto; smt().
 match Cell 1; first auto; smt().
 rcondt 1; first auto; smt().
@@ -1235,21 +883,11 @@ lemma memory_contents_cell_bad (gm : gm , pty' : party, cell_addr' : addr) :
    glob Memory = gm /\ gm_invar (glob Memory) /\
    res = None].
 proof.
-proc.
-if.
-if.
-case
-  (exists (key : key),
-   oget Memory.phys_map.[oget Memory.honest_virt_map.[cell_addr]] =
-   Key key).
-match Key 1; auto.
-match Cell 1; first auto; smt().
-rcondf 1; auto; smt().
-auto.
+proc => /=.
 if.
 case
   (exists (key : key),
-   oget Memory.phys_map.[oget Memory.malicious_virt_map.[cell_addr]] =
+   oget Memory.phys_map.[oget (oget Memory.virt_map.[pty']).[cell_addr]] =
    Key key).
 match Key 1; auto.
 match Cell 1; first auto; smt().
@@ -1443,34 +1081,24 @@ qed.
 lemma party_memory_trans_virt_addr (gm : gm, addr' : addr) :
   hoare
   [PartyMemory.trans_virt_addr :
-   addr = addr' /\
-   (if party = Honest
-    then addr \in Memory.honest_virt_map
-    else addr \in Memory.malicious_virt_map) /\
+   addr = addr' /\ addr \in oget Memory.virt_map.[party] /\
    glob Memory = gm /\ gm_invar gm ==>
    gm_invar (glob Memory) /\
    (* unchanged *)
    Memory.next_key = gm_to_next_key gm /\
    Memory.next_phys_addr = gm_to_next_phys_addr gm /\
    Memory.phys_map = gm_to_phys_map gm /\
+   Memory.next_virt_addr.[party] = (gm_to_next_virt_addr gm).[party] /\
+   Memory.virt_map.[party] = (gm_to_virt_map gm).[party] /\
    (* changed *)
-   if party = Honest
-   then (let phys_addr = oget (Memory.honest_virt_map.[addr']) in
-         let virt_addr_malic = gm_to_malicious_next_virt_addr gm in
-         Memory.honest_next_virt_addr = gm_to_honest_next_virt_addr gm /\
-         Memory.honest_virt_map = gm_to_honest_virt_map gm /\
-         Memory.malicious_next_virt_addr = virt_addr_malic + 1 /\
-         Memory.malicious_virt_map =
-         (gm_to_malicious_virt_map gm).[virt_addr_malic <- phys_addr] /\
-         res = Some virt_addr_malic)
-   else (let phys_addr = oget (Memory.malicious_virt_map.[addr']) in
-         let virt_addr_honest = gm_to_honest_next_virt_addr gm in
-         Memory.malicious_next_virt_addr = gm_to_malicious_next_virt_addr gm /\
-         Memory.malicious_virt_map = gm_to_malicious_virt_map gm /\
-         Memory.honest_next_virt_addr = virt_addr_honest + 1 /\
-         Memory.honest_virt_map =
-         (gm_to_honest_virt_map gm).[virt_addr_honest <- phys_addr] /\
-         res = Some virt_addr_honest)].
+   let phys_addr = oget (oget (Memory.virt_map.[party])).[addr'] in
+   let next_virt_addr_other = oget (gm_to_next_virt_addr gm).[other party] in
+   oget Memory.next_virt_addr.[other party] =
+     next_virt_addr_other + 1 /\
+   oget Memory.virt_map.[other party] =
+   (oget (gm_to_virt_map gm).[other party])
+     .[next_virt_addr_other <- phys_addr] /\
+   res = Some next_virt_addr_other].
 proof.
 proc.
 call (memory_trans_virt_addr gm party addr').
@@ -1499,23 +1127,15 @@ lemma party_memory_create_key (gm : gm) :
    Memory.phys_map =
    (gm_to_phys_map gm)
      .[gm_to_next_phys_addr gm <- Key (gm_to_next_key gm)] /\
-   (if party = Honest
-    then (Memory.honest_next_virt_addr =
-          gm_to_honest_next_virt_addr gm + 1 /\
-          Memory.honest_virt_map =
-          (gm_to_honest_virt_map gm)
-            .[gm_to_honest_next_virt_addr gm <- gm_to_next_phys_addr gm] /\
-          res = gm_to_honest_next_virt_addr gm /\
-          Memory.malicious_next_virt_addr = gm_to_malicious_next_virt_addr gm /\
-          Memory.malicious_virt_map = gm_to_malicious_virt_map gm)
-    else (Memory.malicious_next_virt_addr =
-          gm_to_malicious_next_virt_addr gm + 1 /\
-          Memory.malicious_virt_map =
-          (gm_to_malicious_virt_map gm)
-            .[gm_to_malicious_next_virt_addr gm <- gm_to_next_phys_addr gm] /\
-          res = gm_to_malicious_next_virt_addr gm /\
-          Memory.honest_next_virt_addr = gm_to_honest_next_virt_addr gm /\
-          Memory.honest_virt_map = gm_to_honest_virt_map gm))].
+   oget Memory.next_virt_addr.[party] =
+   oget (gm_to_next_virt_addr gm).[party] + 1 /\
+   oget Memory.virt_map.[party] =
+   (oget (gm_to_virt_map gm).[party])
+     .[oget (gm_to_next_virt_addr gm).[party] <-
+       gm_to_next_phys_addr gm] /\
+   Memory.next_virt_addr.[other party] = (gm_to_next_virt_addr gm).[other party] /\
+   Memory.virt_map.[other party] = (gm_to_virt_map gm).[other party] /\
+   res = oget (gm_to_next_virt_addr gm).[party]].
 proof.
 proc.
 call (memory_create_key gm party).
@@ -1534,23 +1154,15 @@ lemma party_memory_create_key_phl (gm : gm) :
    Memory.phys_map =
    (gm_to_phys_map gm)
      .[gm_to_next_phys_addr gm <- Key (gm_to_next_key gm)] /\
-   (if party = Honest
-    then (Memory.honest_next_virt_addr =
-          gm_to_honest_next_virt_addr gm + 1 /\
-          Memory.honest_virt_map =
-          (gm_to_honest_virt_map gm)
-            .[gm_to_honest_next_virt_addr gm <- gm_to_next_phys_addr gm] /\
-          res = gm_to_honest_next_virt_addr gm /\
-          Memory.malicious_next_virt_addr = gm_to_malicious_next_virt_addr gm /\
-          Memory.malicious_virt_map = gm_to_malicious_virt_map gm)
-    else (Memory.malicious_next_virt_addr =
-          gm_to_malicious_next_virt_addr gm + 1 /\
-          Memory.malicious_virt_map =
-          (gm_to_malicious_virt_map gm)
-            .[gm_to_malicious_next_virt_addr gm <- gm_to_next_phys_addr gm] /\
-          res = gm_to_malicious_next_virt_addr gm /\
-          Memory.honest_next_virt_addr = gm_to_honest_next_virt_addr gm /\
-          Memory.honest_virt_map = gm_to_honest_virt_map gm))] = 1%r.
+   oget Memory.next_virt_addr.[party] =
+   oget (gm_to_next_virt_addr gm).[party] + 1 /\
+   oget Memory.virt_map.[party] =
+   (oget (gm_to_virt_map gm).[party])
+     .[oget (gm_to_next_virt_addr gm).[party] <-
+       gm_to_next_phys_addr gm] /\
+   Memory.next_virt_addr.[other party] = (gm_to_next_virt_addr gm).[other party] /\
+   Memory.virt_map.[other party] = (gm_to_virt_map gm).[other party] /\
+   res = oget (gm_to_next_virt_addr gm).[party]] = 1%r.
 proof.
 conseq (_ : true ==> true) (_ : _ ==> _) => //.
 apply (party_memory_create_key gm).
@@ -1614,33 +1226,20 @@ lemma party_memory_create_cell (gm : gm, key_addr' : addr, b' : bool) :
    gm_invar (glob Memory) /\
    Memory.next_key = gm_to_next_key gm /\
    Memory.next_phys_addr = gm_to_next_phys_addr gm + 1 /\
-   (if party = Honest
-    then (let key = key_addr_to_key Honest gm key_addr' in
-          Memory.phys_map =
-          (gm_to_phys_map gm)
-             .[gm_to_next_phys_addr gm <-
-               Cell {|key = key; cont = b'; locked = true|}] /\
-          Memory.honest_next_virt_addr =
-          gm_to_honest_next_virt_addr gm + 1 /\
-          Memory.honest_virt_map =
-          (gm_to_honest_virt_map gm)
-             .[gm_to_honest_next_virt_addr gm <- gm_to_next_phys_addr gm] /\
-          res = Some (gm_to_honest_next_virt_addr gm) /\
-          Memory.malicious_next_virt_addr = gm_to_malicious_next_virt_addr gm /\
-          Memory.malicious_virt_map = gm_to_malicious_virt_map gm)
-    else (let key = key_addr_to_key Malicious gm key_addr' in
-          Memory.phys_map =
-          (gm_to_phys_map gm)
-             .[gm_to_next_phys_addr gm <-
-               Cell {|key = key; cont = b'; locked = true|}] /\
-          Memory.malicious_next_virt_addr =
-          gm_to_malicious_next_virt_addr gm + 1 /\
-          Memory.malicious_virt_map =
-          (gm_to_malicious_virt_map gm)
-             .[gm_to_malicious_next_virt_addr gm <- gm_to_next_phys_addr gm] /\
-          res = Some (gm_to_malicious_next_virt_addr gm) /\
-          Memory.honest_next_virt_addr = gm_to_honest_next_virt_addr gm /\
-          Memory.honest_virt_map = gm_to_honest_virt_map gm))].
+   Memory.phys_map =
+   (gm_to_phys_map gm)
+      .[gm_to_next_phys_addr gm <-
+        Cell
+        {|key = key_addr_to_key party gm key_addr';
+          cont = b'; locked = true|}] /\
+   oget Memory.next_virt_addr.[party] =
+   oget (gm_to_next_virt_addr gm).[party] + 1 /\
+   oget Memory.virt_map.[party] =
+   (oget (gm_to_virt_map gm).[party])
+      .[oget (gm_to_next_virt_addr gm).[party] <- gm_to_next_phys_addr gm] /\
+   Memory.next_virt_addr.[other party] = (gm_to_next_virt_addr gm).[other party] /\
+   Memory.virt_map.[other party] = (gm_to_virt_map gm).[other party] /\
+   res = Some (oget (gm_to_next_virt_addr gm).[party])].
 proof.
 proc.
 call (memory_create_cell gm party key_addr' b').
@@ -1655,33 +1254,20 @@ lemma party_memory_create_cell_phl (gm : gm, key_addr' : addr, b' : bool) :
    gm_invar (glob Memory) /\
    Memory.next_key = gm_to_next_key gm /\
    Memory.next_phys_addr = gm_to_next_phys_addr gm + 1 /\
-   (if party = Honest
-    then (let key = key_addr_to_key Honest gm key_addr' in
-          Memory.phys_map =
-          (gm_to_phys_map gm)
-             .[gm_to_next_phys_addr gm <-
-               Cell {|key = key; cont = b'; locked = true|}] /\
-          Memory.honest_next_virt_addr =
-          gm_to_honest_next_virt_addr gm + 1 /\
-          Memory.honest_virt_map =
-          (gm_to_honest_virt_map gm)
-             .[gm_to_honest_next_virt_addr gm <- gm_to_next_phys_addr gm] /\
-          res = Some (gm_to_honest_next_virt_addr gm) /\
-          Memory.malicious_next_virt_addr = gm_to_malicious_next_virt_addr gm /\
-          Memory.malicious_virt_map = gm_to_malicious_virt_map gm)
-    else (let key = key_addr_to_key Malicious gm key_addr' in
-          Memory.phys_map =
-          (gm_to_phys_map gm)
-             .[gm_to_next_phys_addr gm <-
-               Cell {|key = key; cont = b'; locked = true|}] /\
-          Memory.malicious_next_virt_addr =
-          gm_to_malicious_next_virt_addr gm + 1 /\
-          Memory.malicious_virt_map =
-          (gm_to_malicious_virt_map gm)
-             .[gm_to_malicious_next_virt_addr gm <- gm_to_next_phys_addr gm] /\
-          res = Some (gm_to_malicious_next_virt_addr gm) /\
-          Memory.honest_next_virt_addr = gm_to_honest_next_virt_addr gm /\
-          Memory.honest_virt_map = gm_to_honest_virt_map gm))] = 1%r.
+   Memory.phys_map =
+   (gm_to_phys_map gm)
+      .[gm_to_next_phys_addr gm <-
+        Cell
+        {|key = key_addr_to_key party gm key_addr';
+          cont = b'; locked = true|}] /\
+   oget Memory.next_virt_addr.[party] =
+   oget (gm_to_next_virt_addr gm).[party] + 1 /\
+   oget Memory.virt_map.[party] =
+   (oget (gm_to_virt_map gm).[party])
+      .[oget (gm_to_next_virt_addr gm).[party] <- gm_to_next_phys_addr gm] /\
+   Memory.next_virt_addr.[other party] = (gm_to_next_virt_addr gm).[other party] /\
+   Memory.virt_map.[other party] = (gm_to_virt_map gm).[other party] /\
+   res = Some (oget (gm_to_next_virt_addr gm).[party])] = 1%r.
 proof.
 conseq (_ : true ==> true) (_ : _ ==> _) => //.
 apply (party_memory_create_cell gm key_addr' b').
@@ -1747,33 +1333,20 @@ lemma party_memory_unlock_cell (gm : gm , cell_addr' key_addr' : addr) :
    gm_invar (glob Memory) /\
    Memory.next_key = gm_to_next_key gm /\
    Memory.next_phys_addr = gm_to_next_phys_addr gm + 1 /\
-   (if party = Honest
-    then (let cell = cell_addr_to_cell Honest gm cell_addr' in
-          Memory.phys_map =
-          (gm_to_phys_map gm)
-             .[gm_to_next_phys_addr gm <-
-               Cell {|cell with locked = false|}] /\
-          Memory.honest_next_virt_addr =
-          gm_to_honest_next_virt_addr gm + 1 /\
-          Memory.honest_virt_map =
-          (gm_to_honest_virt_map gm)
-             .[gm_to_honest_next_virt_addr gm <- gm_to_next_phys_addr gm] /\
-          res = Some (gm_to_honest_next_virt_addr gm) /\
-          Memory.malicious_next_virt_addr = gm_to_malicious_next_virt_addr gm /\
-          Memory.malicious_virt_map = gm_to_malicious_virt_map gm)
-    else (let cell = cell_addr_to_cell Malicious gm cell_addr' in
-          Memory.phys_map =
-          (gm_to_phys_map gm)
-             .[gm_to_next_phys_addr gm <-
-               Cell {|cell with locked = false|}] /\
-          Memory.malicious_next_virt_addr =
-          gm_to_malicious_next_virt_addr gm + 1 /\
-          Memory.malicious_virt_map =
-          (gm_to_malicious_virt_map gm)
-             .[gm_to_malicious_next_virt_addr gm <- gm_to_next_phys_addr gm] /\
-          res = Some (gm_to_malicious_next_virt_addr gm) /\
-          Memory.honest_next_virt_addr = gm_to_honest_next_virt_addr gm /\
-          Memory.honest_virt_map = gm_to_honest_virt_map gm))].
+   Memory.phys_map =
+   (gm_to_phys_map gm)
+     .[gm_to_next_phys_addr gm <-
+       Cell
+       {|(cell_addr_to_cell party gm cell_addr') with locked = false|}] /\
+   oget Memory.next_virt_addr.[party] =
+   oget (gm_to_next_virt_addr gm).[party] + 1 /\
+   oget Memory.virt_map.[party] =
+   (oget (gm_to_virt_map gm).[party])
+     .[oget (gm_to_next_virt_addr gm).[party] <- gm_to_next_phys_addr gm] /\
+   Memory.next_virt_addr.[other party] = 
+   (gm_to_next_virt_addr gm).[other party] /\
+   Memory.virt_map.[other party] =  (gm_to_virt_map gm).[other party] /\
+   res = Some (oget (gm_to_next_virt_addr gm).[party])].
 proof.
 proc.
 call (memory_unlock_cell gm party cell_addr' key_addr').
@@ -2290,13 +1863,10 @@ local lemma Exper_distinguish :
     then OtherHonest.HPS_Guesser_WaitFromAdvGuess
     else OtherHonest.HPS_Chooser_WaitFromAdvChoice) /\
    gm_invar (glob Memory) /\
-   Memory.next_key = 0 /\
-   Memory.next_phys_addr = 0 /\
+   Memory.next_key = 0 /\ Memory.next_phys_addr = 0 /\
    Memory.phys_map = empty /\
-   Memory.honest_next_virt_addr = 0 /\
-   Memory.honest_virt_map = empty /\
-   Memory.malicious_next_virt_addr = 0 /\
-   Memory.malicious_virt_map = empty ==>
+   Memory.next_virt_addr = empty.[Honest <- 0].[Malicious <- 0] /\
+   Memory.virt_map       = empty.[Honest <- empty].[Malicious <- empty] ==>
    res].
 proof.
 proc.
@@ -2322,14 +1892,14 @@ seq 1 :
       .[0 <- Key 0]
       .[1 <- Cell {|key = 0; cont = choice; locked = true|}] /\
   (if CorrectAdv.chooser = Honest
-   then (Memory.honest_next_virt_addr = 2 /\
-         Memory.honest_virt_map = (empty.[0 <- 0]).[1 <- 1] /\
-         Memory.malicious_next_virt_addr = 0 /\
-         Memory.malicious_virt_map = empty)
-   else (Memory.malicious_next_virt_addr = 2 /\
-         Memory.malicious_virt_map = (empty.[0 <- 0]).[1 <- 1] /\
-         Memory.honest_next_virt_addr = 0 /\
-         Memory.honest_virt_map = empty))).
+   then (oget Memory.next_virt_addr.[Honest] = 2 /\
+         oget Memory.virt_map.[Honest] = (empty.[0 <- 0]).[1 <- 1] /\
+         oget Memory.next_virt_addr.[Malicious] = 0 /\
+         oget Memory.virt_map.[Malicious] = empty)
+   else (oget Memory.next_virt_addr.[Malicious] = 2 /\
+         oget Memory.virt_map.[Malicious] = (empty.[0 <- 0]).[1 <- 1] /\
+         oget Memory.next_virt_addr.[Honest] = 0 /\
+         oget Memory.virt_map.[Honest] = empty))).
 inline RealProtocol(Honest.Honest, OtherHonest.Honest).from_adv.
 sp.
 match.
@@ -2348,12 +1918,13 @@ seq 1 :
    key_addr = 0 /\ gm_invar (glob Memory) /\
    Memory.next_key = 1 /\ Memory.next_phys_addr = 1 /\
    Memory.phys_map = empty.[0 <- Key 0] /\
-   Memory.honest_next_virt_addr = 1 /\
-   Memory.honest_virt_map = (empty.[0 <- 0]) /\
-   Memory.malicious_next_virt_addr = 0 /\
-   Memory.malicious_virt_map = empty).
+   oget Memory.next_virt_addr.[Honest] = 1 /\
+   oget Memory.virt_map.[Honest] = empty.[0 <- 0] /\
+   oget Memory.next_virt_addr.[Malicious] = 0 /\
+   oget Memory.virt_map.[Malicious] = empty).
 exlim (glob Memory) => gm.
-call (HonestMemory.party_memory_create_key gm); first auto.
+call (HonestMemory.party_memory_create_key gm).
+auto; progress [-delta]; smt(get_setE).
 exlim (glob Memory) => gm'.
 exlim choice0 => ch.
 call (HonestMemory.party_memory_create_cell gm' 0 ch).
@@ -2373,12 +1944,12 @@ seq 1 :
    key_addr = 0 /\ gm_invar (glob Memory) /\
    Memory.next_key = 1 /\ Memory.next_phys_addr = 1 /\
    Memory.phys_map = empty.[0 <- Key 0] /\
-   Memory.malicious_next_virt_addr = 1 /\
-   Memory.malicious_virt_map = (empty.[0 <- 0]) /\
-   Memory.honest_next_virt_addr = 0 /\
-   Memory.honest_virt_map = empty).
+   oget Memory.next_virt_addr.[Malicious] = 1 /\
+   oget Memory.virt_map.[Malicious] = empty.[0 <- 0] /\
+   oget Memory.next_virt_addr.[Honest] = 0 /\
+   oget Memory.virt_map.[Honest] = empty).
 exlim (glob Memory) => gm.
-call (MaliciousMemory.party_memory_create_key gm); first auto.
+call (MaliciousMemory.party_memory_create_key gm); first auto; smt(get_setE).
 exlim (glob Memory) => gm'.
 exlim choice0 => ch.
 call (MaliciousMemory.party_memory_create_cell gm' 0 ch).
@@ -2404,14 +1975,14 @@ seq 1 :
        .[0 <- Key 0]
        .[1 <- Cell {|key = 0; cont = choice; locked = true|}] /\
    (if CorrectAdv.chooser = Honest
-    then (Memory.honest_next_virt_addr = 2 /\
-          Memory.honest_virt_map = (empty.[0 <- 0]).[1 <- 1] /\
-          Memory.malicious_next_virt_addr = 0 /\
-          Memory.malicious_virt_map = empty)
-    else (Memory.malicious_next_virt_addr = 2 /\
-          Memory.malicious_virt_map = (empty.[0 <- 0]).[1 <- 1] /\
-          Memory.honest_next_virt_addr = 0 /\
-          Memory.honest_virt_map = empty))).
+    then (oget Memory.next_virt_addr.[Honest] = 2 /\
+          oget Memory.virt_map.[Honest] = empty.[0 <- 0].[1 <- 1] /\
+          oget Memory.next_virt_addr.[Malicious] = 0 /\
+          oget Memory.virt_map.[Malicious] = empty)
+    else (oget Memory.next_virt_addr.[Malicious] = 2 /\
+          oget Memory.virt_map.[Malicious] = empty.[0 <- 0].[1 <- 1] /\
+          oget Memory.next_virt_addr.[Honest] = 0 /\
+          oget Memory.virt_map.[Honest] = empty))).
 inline RealProtocol(Honest.Honest, OtherHonest.Honest).from_adv.
 sp.
 match.
@@ -2447,14 +2018,14 @@ seq 1 :
        .[0 <- Key 0]
        .[1 <- Cell {|key = 0; cont = choice; locked = true|}] /\
    (if CorrectAdv.chooser = Honest
-    then (Memory.honest_next_virt_addr = 2 /\
-          Memory.honest_virt_map = (empty.[0 <- 0]).[1 <- 1] /\
-          Memory.malicious_next_virt_addr = 1 /\
-          Memory.malicious_virt_map = empty.[0 <- 1])
-    else (Memory.malicious_next_virt_addr = 2 /\
-          Memory.malicious_virt_map = (empty.[0 <- 0]).[1 <- 1] /\
-          Memory.honest_next_virt_addr = 1 /\
-          Memory.honest_virt_map = empty.[0 <- 1]))).
+    then (oget Memory.next_virt_addr.[Honest] = 2 /\
+          oget Memory.virt_map.[Honest] = empty.[0 <- 0].[1 <- 1] /\
+          oget Memory.next_virt_addr.[Malicious] = 1 /\
+          oget Memory.virt_map.[Malicious] = empty.[0 <- 1])
+    else (oget Memory.next_virt_addr.[Malicious] = 2 /\
+          oget Memory.virt_map.[Malicious] = empty.[0 <- 0].[1 <- 1] /\
+          oget Memory.next_virt_addr.[Honest] = 1 /\
+          oget Memory.virt_map.[Honest] = empty.[0 <- 1]))).
 inline RealProtocol(Honest.Honest, OtherHonest.Honest).queue.
 sp.
 match.
@@ -2496,14 +2067,14 @@ seq 1 :
        .[0 <- Key 0]
        .[1 <- Cell {|key = 0; cont = choice; locked = true|}] /\
    (if CorrectAdv.chooser = Honest
-    then (Memory.honest_next_virt_addr = 2 /\
-          Memory.honest_virt_map = (empty.[0 <- 0]).[1 <- 1] /\
-          Memory.malicious_next_virt_addr = 1 /\
-          Memory.malicious_virt_map = empty.[0 <- 1])
-    else (Memory.malicious_next_virt_addr = 2 /\
-          Memory.malicious_virt_map = (empty.[0 <- 0]).[1 <- 1] /\
-          Memory.honest_next_virt_addr = 1 /\
-          Memory.honest_virt_map = empty.[0 <- 1]))).
+    then (oget Memory.next_virt_addr.[Honest] = 2 /\
+          oget Memory.virt_map.[Honest] = empty.[0 <- 0].[1 <- 1] /\
+          oget Memory.next_virt_addr.[Malicious] = 1 /\
+          oget Memory.virt_map.[Malicious] = empty.[0 <- 1])
+    else (oget Memory.next_virt_addr.[Malicious] = 2 /\
+          oget Memory.virt_map.[Malicious] = empty.[0 <- 0].[1 <- 1] /\
+          oget Memory.next_virt_addr.[Honest] = 1 /\
+          oget Memory.virt_map.[Honest] = empty.[0 <- 1]))).
 inline RealProtocol(Honest.Honest, OtherHonest.Honest).deliver.
 sp.
 match.
@@ -2549,14 +2120,14 @@ seq 1 :
        .[0 <- Key 0]
        .[1 <- Cell {|key = 0; cont = choice; locked = true|}] /\
    (if CorrectAdv.chooser = Honest
-    then (Memory.honest_next_virt_addr = 2 /\
-          Memory.honest_virt_map = (empty.[0 <- 0]).[1 <- 1] /\
-          Memory.malicious_next_virt_addr = 1 /\
-          Memory.malicious_virt_map = empty.[0 <- 1])
-    else (Memory.malicious_next_virt_addr = 2 /\
-          Memory.malicious_virt_map = (empty.[0 <- 0]).[1 <- 1] /\
-          Memory.honest_next_virt_addr = 1 /\
-          Memory.honest_virt_map = empty.[0 <- 1]))).
+    then (oget Memory.next_virt_addr.[Honest] = 2 /\
+          oget Memory.virt_map.[Honest] = empty.[0 <- 0].[1 <- 1] /\
+          oget Memory.next_virt_addr.[Malicious] = 1 /\
+          oget Memory.virt_map.[Malicious] = empty.[0 <- 1])
+    else (oget Memory.next_virt_addr.[Malicious] = 2 /\
+          oget Memory.virt_map.[Malicious] = empty.[0 <- 0].[1 <- 1] /\
+          oget Memory.next_virt_addr.[Honest] = 1 /\
+          oget Memory.virt_map.[Honest] = empty.[0 <- 1]))).
 inline RealProtocol(Honest.Honest, OtherHonest.Honest).queue.
 sp.
 match.
@@ -2592,14 +2163,14 @@ seq 1 :
        .[0 <- Key 0]
        .[1 <- Cell {|key = 0; cont = choice; locked = true|}] /\
    (if CorrectAdv.chooser = Honest
-    then (Memory.honest_next_virt_addr = 2 /\
-          Memory.honest_virt_map = (empty.[0 <- 0]).[1 <- 1] /\
-          Memory.malicious_next_virt_addr = 1 /\
-          Memory.malicious_virt_map = empty.[0 <- 1])
-    else (Memory.malicious_next_virt_addr = 2 /\
-          Memory.malicious_virt_map = (empty.[0 <- 0]).[1 <- 1] /\
-          Memory.honest_next_virt_addr = 1 /\
-          Memory.honest_virt_map = empty.[0 <- 1]))).
+    then (oget Memory.next_virt_addr.[Honest] = 2 /\
+          oget Memory.virt_map.[Honest] = empty.[0 <- 0].[1 <- 1] /\
+          oget Memory.next_virt_addr.[Malicious] = 1 /\
+          oget Memory.virt_map.[Malicious] = empty.[0 <- 1])
+    else (oget Memory.next_virt_addr.[Malicious] = 2 /\
+          oget Memory.virt_map.[Malicious] = empty.[0 <- 0].[1 <- 1] /\
+          oget Memory.next_virt_addr.[Honest] = 1 /\
+          oget Memory.virt_map.[Honest] = empty.[0 <- 1]))).
 inline RealProtocol(Honest.Honest, OtherHonest.Honest).deliver.
 sp.
 match.
@@ -2639,14 +2210,14 @@ seq 1 :
        .[0 <- Key 0]
        .[1 <- Cell {|key = 0; cont = choice; locked = true|}] /\
    (if CorrectAdv.chooser = Honest
-    then (Memory.honest_next_virt_addr = 2 /\
-          Memory.honest_virt_map = (empty.[0 <- 0]).[1 <- 1] /\
-          Memory.malicious_next_virt_addr = 2 /\
-          Memory.malicious_virt_map = empty.[0 <- 1].[1 <- 0])
-    else (Memory.malicious_next_virt_addr = 2 /\
-          Memory.malicious_virt_map = (empty.[0 <- 0]).[1 <- 1] /\
-          Memory.honest_next_virt_addr = 2 /\
-          Memory.honest_virt_map = empty.[0 <- 1].[1 <- 0]))).
+    then (oget Memory.next_virt_addr.[Honest] = 2 /\
+          oget Memory.virt_map.[Honest] = empty.[0 <- 0].[1 <- 1] /\
+          oget Memory.next_virt_addr.[Malicious] = 2 /\
+          oget Memory.virt_map.[Malicious] = empty.[0 <- 1].[1 <- 0])
+    else (oget Memory.next_virt_addr.[Malicious] = 2 /\
+          oget Memory.virt_map.[Malicious] = empty.[0 <- 0].[1 <- 1] /\
+          oget Memory.next_virt_addr.[Honest] = 2 /\
+          oget Memory.virt_map.[Honest] = empty.[0 <- 1].[1 <- 0]))).
 inline RealProtocol(Honest.Honest, OtherHonest.Honest).queue.
 sp.
 match.
@@ -2687,14 +2258,14 @@ seq 1 :
        .[1 <- Cell {|key = 0; cont = choice; locked = true|}]
        .[2 <- Cell {|key = 0; cont = choice; locked = false|}] /\
    (if CorrectAdv.chooser = Honest
-    then (Memory.honest_next_virt_addr = 2 /\
-          Memory.honest_virt_map = (empty.[0 <- 0]).[1 <- 1] /\
-          Memory.malicious_next_virt_addr = 3 /\
-          Memory.malicious_virt_map = empty.[0 <- 1].[1 <- 0].[2 <- 2])
-    else (Memory.malicious_next_virt_addr = 2 /\
-          Memory.malicious_virt_map = (empty.[0 <- 0]).[1 <- 1] /\
-          Memory.honest_next_virt_addr = 3 /\
-          Memory.honest_virt_map = empty.[0 <- 1].[1 <- 0].[2 <- 2]))).
+    then (oget Memory.next_virt_addr.[Honest] = 2 /\
+          oget Memory.virt_map.[Honest] = empty.[0 <- 0].[1 <- 1] /\
+          oget Memory.next_virt_addr.[Malicious] = 3 /\
+          oget Memory.virt_map.[Malicious] = empty.[0 <- 1].[1 <- 0].[2 <- 2])
+    else (oget Memory.next_virt_addr.[Malicious] = 2 /\
+          oget Memory.virt_map.[Malicious] = empty.[0 <- 0].[1 <- 1] /\
+          oget Memory.next_virt_addr.[Honest] = 3 /\
+          oget Memory.virt_map.[Honest] = empty.[0 <- 1].[1 <- 0].[2 <- 2]))).
 inline RealProtocol(Honest.Honest, OtherHonest.Honest).deliver.
 sp.
 match.
@@ -2721,13 +2292,13 @@ seq 1 :
        .[0 <- Key 0]
        .[1 <- Cell {|key = 0; cont = choice; locked = true|}]
        .[2 <- Cell {|key = 0; cont = choice; locked = false|}] /\
-    (Memory.malicious_next_virt_addr = 2 /\
-     Memory.malicious_virt_map = (empty.[0 <- 0]).[1 <- 1] /\
-     Memory.honest_next_virt_addr = 3 /\
-     Memory.honest_virt_map = empty.[0 <- 1].[1 <- 0].[2 <- 2])).
+    (oget Memory.next_virt_addr.[Malicious] = 2 /\
+     oget Memory.virt_map.[Malicious] = empty.[0 <- 0].[1 <- 1] /\
+     oget Memory.next_virt_addr.[Honest] = 3 /\
+     oget Memory.virt_map.[Honest] = empty.[0 <- 1].[1 <- 0].[2 <- 2])).
 exlim (glob Memory) => gm.
 call (HonestMemory.party_memory_unlock_cell gm 0 1).
-auto; smt(mem_set get_setE).
+auto; smt(mem_set get_setE oget_some).
 match Some 1; first auto; smt().
 wp.
 exlim (glob Memory) => gm.
@@ -2757,10 +2328,10 @@ seq 1 :
        .[0 <- Key 0]
        .[1 <- Cell {|key = 0; cont = choice; locked = true|}]
        .[2 <- Cell {|key = 0; cont = choice; locked = false|}] /\
-    (Memory.honest_next_virt_addr = 2 /\
-     Memory.honest_virt_map = (empty.[0 <- 0]).[1 <- 1] /\
-     Memory.malicious_next_virt_addr = 3 /\
-     Memory.malicious_virt_map = empty.[0 <- 1].[1 <- 0].[2 <- 2])).
+    (oget Memory.next_virt_addr.[Honest] = 2 /\
+     oget Memory.virt_map.[Honest] = empty.[0 <- 0].[1 <- 1] /\
+     oget Memory.next_virt_addr.[Malicious] = 3 /\
+     oget Memory.virt_map.[Malicious] = empty.[0 <- 1].[1 <- 0].[2 <- 2])).
 exlim (glob Memory) => gm.
 call (MaliciousMemory.party_memory_unlock_cell gm 0 1).
 auto; progress; smt(mem_set get_setE).
@@ -2794,14 +2365,14 @@ seq 1 :
        .[1 <- Cell {|key = 0; cont = choice; locked = true|}]
        .[2 <- Cell {|key = 0; cont = choice; locked = false|}] /\
    (if CorrectAdv.chooser = Honest
-    then (Memory.honest_next_virt_addr = 2 /\
-          Memory.honest_virt_map = (empty.[0 <- 0]).[1 <- 1] /\
-          Memory.malicious_next_virt_addr = 3 /\
-          Memory.malicious_virt_map = empty.[0 <- 1].[1 <- 0].[2 <- 2])
-    else (Memory.malicious_next_virt_addr = 2 /\
-          Memory.malicious_virt_map = (empty.[0 <- 0]).[1 <- 1] /\
-          Memory.honest_next_virt_addr = 3 /\
-          Memory.honest_virt_map = empty.[0 <- 1].[1 <- 0].[2 <- 2]))).
+    then (oget Memory.next_virt_addr.[Honest] = 2 /\
+          oget Memory.virt_map.[Honest] = empty.[0 <- 0].[1 <- 1] /\
+          oget Memory.next_virt_addr.[Malicious] = 3 /\
+          oget Memory.virt_map.[Malicious] = empty.[0 <- 1].[1 <- 0].[2 <- 2])
+    else (oget Memory.next_virt_addr.[Malicious] = 2 /\
+          oget Memory.virt_map.[Malicious] = empty.[0 <- 0].[1 <- 1] /\
+          oget Memory.next_virt_addr.[Honest] = 3 /\
+          oget Memory.virt_map.[Honest] = empty.[0 <- 1].[1 <- 0].[2 <- 2]))).
 inline RealProtocol(Honest.Honest, OtherHonest.Honest).to_adv.
 sp.
 match.
@@ -2838,14 +2409,14 @@ seq 1 :
        .[1 <- Cell {|key = 0; cont = choice; locked = true|}]
        .[2 <- Cell {|key = 0; cont = choice; locked = false|}] /\
    (if CorrectAdv.chooser = Honest
-    then (Memory.honest_next_virt_addr = 2 /\
-          Memory.honest_virt_map = (empty.[0 <- 0]).[1 <- 1] /\
-          Memory.malicious_next_virt_addr = 3 /\
-          Memory.malicious_virt_map = empty.[0 <- 1].[1 <- 0].[2 <- 2])
-    else (Memory.malicious_next_virt_addr = 2 /\
-          Memory.malicious_virt_map = (empty.[0 <- 0]).[1 <- 1] /\
-          Memory.honest_next_virt_addr = 3 /\
-          Memory.honest_virt_map = empty.[0 <- 1].[1 <- 0].[2 <- 2]))).
+    then (oget Memory.next_virt_addr.[Honest] = 2 /\
+          oget Memory.virt_map.[Honest] = empty.[0 <- 0].[1 <- 1] /\
+          oget Memory.next_virt_addr.[Malicious] = 3 /\
+          oget Memory.virt_map.[Malicious] = empty.[0 <- 1].[1 <- 0].[2 <- 2])
+    else (oget Memory.next_virt_addr.[Malicious] = 2 /\
+          oget Memory.virt_map.[Malicious] = empty.[0 <- 0].[1 <- 1] /\
+          oget Memory.next_virt_addr.[Honest] = 3 /\
+          oget Memory.virt_map.[Honest] = empty.[0 <- 1].[1 <- 0].[2 <- 2]))).
 inline RealProtocol(Honest.Honest, OtherHonest.Honest).to_adv.
 sp.
 match.
@@ -2891,13 +2462,10 @@ seq 1 :
       then OtherHonest.HPS_Guesser_WaitFromAdvGuess
       else OtherHonest.HPS_Chooser_WaitFromAdvChoice) /\
    gm_invar (glob Memory) /\
-   Memory.next_key                 = 0 /\
-   Memory.next_phys_addr           = 0 /\
-   Memory.phys_map                 = empty /\
-   Memory.honest_next_virt_addr    = 0 /\
-   Memory.honest_virt_map          = empty /\
-   Memory.malicious_next_virt_addr = 0 /\
-   Memory.malicious_virt_map       = empty).
+   Memory.next_key = 0 /\ Memory.next_phys_addr = 0 /\
+   Memory.phys_map = empty /\
+   Memory.next_virt_addr = empty.[Honest <- 0].[Malicious <- 0] /\
+   Memory.virt_map       = empty.[Honest <- empty].[Malicious <- empty]).
 inline RealProtocol(Honest.Honest, OtherHonest.Honest).init.
 call memory_init.
 sp.
@@ -3408,9 +2976,10 @@ qed.
 op gm_invar_guesser
    (gm : gm, cell_hon_virt_addr cell_phys_addr : addr, cont : bool) : bool =
   exists (key : key, locked : bool),
-  (gm_to_honest_virt_map gm).[cell_hon_virt_addr] = Some cell_phys_addr /\
+  (oget (gm_to_virt_map gm).[Honest]).[cell_hon_virt_addr] =
+  Some cell_phys_addr /\
   (gm_to_phys_map gm).[cell_phys_addr] =
-    Some (Cell {|key = key; cont = cont; locked = locked|}).
+  Some (Cell {|key = key; cont = cont; locked = locked|}).
 
 lemma malic_trans_virt_addr_gm_invar_guesser_equiv
       (cell_hon_virt_addr cell_phys_addr : addr, cont : bool) :
@@ -3436,14 +3005,13 @@ conseq
    cont)
   (_ : true ==> true) => //.
 proc; inline*; sp 2.
-rcondf 1; first auto.
 if.
 auto; progress.
 rewrite /gm_invar_guesser /gm_to_honest_virt_map /gm_to_phys_map /=.
 rewrite /gm_invar_guesser in H0.
 elim H0 => key locked H0.
 exists key locked.
-smt(get_setE).
+smt(get_setE oget_some).
 auto.
 apply malic_trans_virt_addr_gm_invar_equiv.
 qed.
@@ -3783,28 +3351,30 @@ qed.
 op gm_rel_invar_chooser
    (gm1 gm2 : gm, cell_hon_virt_addr cell_phys_addr : addr, key : key,
     cont : bool) : bool =
-  gm_to_next_key gm1                 = gm_to_next_key gm2                 /\
-  gm_to_next_phys_addr gm1           = gm_to_next_phys_addr gm2           /\
-  gm_to_honest_next_virt_addr gm1    = gm_to_honest_next_virt_addr gm2    /\
-  gm_to_honest_virt_map gm1          = gm_to_honest_virt_map gm2          /\
-  gm_to_malicious_next_virt_addr gm1 = gm_to_malicious_next_virt_addr gm2 /\
-  gm_to_malicious_virt_map gm1       = gm_to_malicious_virt_map gm2       /\
-  (* *)
-  fdom (gm_to_phys_map gm1) = fdom (gm_to_phys_map gm2)                   /\
-  (gm_to_honest_virt_map gm1).[cell_hon_virt_addr] = Some cell_phys_addr  /\
-  (gm_to_phys_map gm1).[cell_phys_addr] =
-  Some (Cell {|key = key; cont = cont; locked = true|})                   /\
-  (gm_to_phys_map gm2).[cell_phys_addr] =
-  Some (Cell {|key = key; cont = true; locked = true|})                   /\
-  (* *)
+  gm_to_next_key gm1        = gm_to_next_key gm2              /\
+  gm_to_next_phys_addr gm1  = gm_to_next_phys_addr gm2        /\
+  gm_to_next_virt_addr gm1  = gm_to_next_virt_addr gm2        /\
+  gm_to_virt_map gm1        = gm_to_virt_map gm2              /\
+  fdom (gm_to_phys_map gm1) = fdom (gm_to_phys_map gm2)       /\
   (forall (phys_addr' : addr),
-   phys_addr' \in gm_to_phys_map gm1 => phys_addr' <> cell_phys_addr =>
+   phys_addr' \in gm_to_phys_map gm1 =>
+   phys_addr' <> cell_phys_addr =>
    (gm_to_phys_map gm1).[phys_addr'] =
-   (gm_to_phys_map gm2).[phys_addr'])                                     /\
+   (gm_to_phys_map gm2).[phys_addr'])                         /\
+  (* *)
+  (oget (gm_to_virt_map gm1).[Honest])
+    .[cell_hon_virt_addr] = Some cell_phys_addr               /\
+  (gm_to_phys_map gm1).[cell_phys_addr] =
+  Some (Cell {|key = key; cont = cont; locked = true|})       /\
+  (gm_to_phys_map gm2).[cell_phys_addr] =
+  Some (Cell {|key = key; cont = true; locked = true|})       /\
+  (* *)
   (forall (mal_virt_addr : addr),
-   mal_virt_addr \in gm_to_malicious_virt_map gm1 =>
+   mal_virt_addr \in oget (gm_to_virt_map gm1).[Malicious] =>
    let phys_addr' =
-     oget (gm_to_malicious_virt_map gm1).[mal_virt_addr] in
+     oget
+     (oget (gm_to_virt_map gm1).[Malicious])
+       .[mal_virt_addr] in
    oget (gm_to_phys_map gm1).[phys_addr'] <> Key key).
 
 lemma gm_rel_invar_chooser_malic_key_not_accessible_gm2
@@ -3813,10 +3383,12 @@ lemma gm_rel_invar_chooser_malic_key_not_accessible_gm2
   gm_invar gm1 =>
   gm_rel_invar_chooser gm1 gm2 cell_hon_virt_addr cell_phys_addr key cont =>
   (forall (mal_virt_addr : addr),
-   mal_virt_addr \in gm_to_malicious_virt_map gm2 =>
+   mal_virt_addr \in oget (gm_to_virt_map gm2).[Malicious] =>
    let phys_addr' =
-     oget (gm_to_malicious_virt_map gm2).[mal_virt_addr] in
-   oget (gm_to_phys_map gm2).[phys_addr'] <> Key key).
+     oget
+     (oget (gm_to_virt_map gm2).[Malicious])
+       .[mal_virt_addr] in
+   oget (gm_to_phys_map gm1).[phys_addr'] <> Key key).
 proof. smt(). qed.
 
 lemma malic_trans_virt_addr_gm_rel_invar_chooser_equiv
@@ -3847,12 +3419,7 @@ conseq
 apply MaliciousMemory.party_memory_trans_virt_addr_gm_invar.
 apply MaliciousMemory.party_memory_trans_virt_addr_gm_invar.
 proc; inline*; sp 2 2.
-if => //.
-auto.
-if => //.
-auto; progress; smt(get_setE).
-auto; progress; smt(get_setE).
-auto.
+(if; first smt()); auto; progress; smt(get_setE oget_some).
 qed.
 
 lemma malic_create_key_gm_rel_invar_chooser_equiv
@@ -3910,7 +3477,7 @@ conseq
   (_ : gm_invar (glob Memory) ==> gm_invar (glob Memory)) => //.
 apply MaliciousMemory.party_memory_is_key_gm_invar.
 apply MaliciousMemory.party_memory_is_key_gm_invar.
-proc; inline*; auto; smt().
+proc; inline*; auto; smt(mem_fdom).
 qed.
 
 lemma malic_create_cell_gm_rel_invar_chooser_equiv
@@ -3941,14 +3508,10 @@ conseq
 apply MaliciousMemory.party_memory_create_cell_gm_invar.
 apply MaliciousMemory.party_memory_create_cell_gm_invar.
 proc; inline*; sp 3 3.
-if => //.
-if => //.
-auto.
-auto.
 if; first smt().
-match; first 2 smt().
+match; first 2 smt(mem_fdom).
 move => key1 key2.
-auto; smt(get_setE fdom_set).
+auto; progress; smt(get_setE fdom_set mem_fdom).
 move => cell1 cell2.
 auto.
 auto.
@@ -3981,7 +3544,7 @@ conseq
   (_ : gm_invar (glob Memory) ==> gm_invar (glob Memory)) => //.
 apply MaliciousMemory.party_memory_is_cell_gm_invar.
 apply MaliciousMemory.party_memory_is_cell_gm_invar.
-proc; inline*; auto; smt().
+proc; inline*; auto; smt(mem_fdom).
 qed.
 
 lemma malic_unlock_cell_gm_rel_invar_chooser_equiv
@@ -4012,31 +3575,23 @@ conseq
 apply MaliciousMemory.party_memory_unlock_cell_gm_invar.
 apply MaliciousMemory.party_memory_unlock_cell_gm_invar.
 proc; inline*; sp 3 3.
-if => //.
-auto.
 if; first smt().
 sp 2 2.
-if; first smt().
+if; first smt(mem_fdom).
 sp 2 2.
-if; first smt().
-auto; progress; first 7 smt().
-smt(get_setE fdom_set).
-smt().
-smt(get_setE fdom_set).
-smt(get_setE fdom_set).
+if; first smt(mem_fdom).
+(auto; progress; first 6 smt(get_setE fdom_set mem_fdom fdomP));
+  last 4 smt(get_setE fdom_set mem_fdom fdomP).
 rewrite /gm_to_phys_map /=.
 case (phys_addr' = Memory.next_phys_addr{1}) => [eq_pa'_npa | neq_pa'_npa].
 rewrite 2!get_setE eq_pa'_npa.
 have -> // : Memory.next_phys_addr{2} = Memory.next_phys_addr{1}.
-smt(). smt().
+smt(). smt(mem_fdom).
 rewrite 2!get_setE.
 have -> /= : Memory.next_phys_addr{2} = Memory.next_phys_addr{1}.
 smt().
 rewrite neq_pa'_npa /=; smt(fdomP).
-smt(get_setE).
-auto.
-auto.
-auto.
+auto. auto. auto.
 qed.
 
 lemma malic_contents_cell_gm_rel_invar_chooser_equiv
@@ -4066,7 +3621,7 @@ conseq
   (_ : gm_invar (glob Memory) ==> gm_invar (glob Memory)) => //.
 apply MaliciousMemory.party_memory_contents_cell_gm_invar.
 apply MaliciousMemory.party_memory_contents_cell_gm_invar.
-proc; inline*; auto; smt().
+proc; inline*; auto; smt(mem_fdom).
 qed.
 
 lemma malicious_party_gm_rel_invar_chooser_from_adv
@@ -4292,9 +3847,7 @@ apply HonestMemory.party_memory_trans_virt_addr_gm_invar.
 proc; inline*; sp 2 2.
 rcondt{1} 1; first auto; smt().
 rcondt{2} 1; first auto; smt().
-if; first smt().
 auto; smt(get_setE).
-auto.
 qed.
 
 (* extra procedures for honest party of simulator *)
@@ -4317,8 +3870,8 @@ module ExtraHonestMemorySim : EXTRA_HONEST_MEMORY_SIM = {
   proc modify_cell(cell_addr : addr, b : bool) : unit = {
     var r : bool; var phys_addr, virt_addr : addr;
     var obj_cell; var new_cell : cell;
-    if (cell_addr \in Memory.honest_virt_map) {
-      phys_addr <- oget Memory.honest_virt_map.[cell_addr];
+    if (cell_addr \in oget Memory.virt_map.[Honest]) {
+      phys_addr <- oget (oget Memory.virt_map.[Honest]).[cell_addr];
       obj_cell <- oget Memory.phys_map.[phys_addr];
       match obj_cell with
       | Key _     => { }
@@ -4333,8 +3886,8 @@ module ExtraHonestMemorySim : EXTRA_HONEST_MEMORY_SIM = {
   proc read_cell(cell_addr : addr) : bool option = {
     var r : bool option;  var phys_addr, virt_addr : addr;
     var obj_cell; var cell : cell;
-    if (cell_addr \in Memory.honest_virt_map) {
-      phys_addr <- oget Memory.honest_virt_map.[cell_addr];
+    if (cell_addr \in oget Memory.virt_map.[Honest]) {
+      phys_addr <- oget (oget Memory.virt_map.[Honest]).[cell_addr];
       obj_cell <- oget Memory.phys_map.[phys_addr];
       match obj_cell with
       | Key _     => { r <- None; }
@@ -4361,10 +3914,10 @@ proc => /=.
 if.
 sp.
 match Cell 1; first auto; smt().
-auto; progress; (apply gm_eqP; first 2 smt()); last 4 smt().
+(auto; progress; apply gm_eqP; first 2 smt()); last 2 smt().
 rewrite /gm_to_phys_map /=.
 have -> :
-  oget Memory.honest_virt_map{hr}.[cell_addr{hr}] =
+  oget (oget Memory.virt_map{hr}.[Honest]).[cell_addr{hr}] =
   cell_phys_addr by smt().
 have doms_eq :
   fdom (gm_to_phys_map gm1) = fdom Memory.phys_map{hr} by smt().
@@ -4392,7 +3945,6 @@ lemma is_cell_read_cell_good (gm : gm, cell_addr' : addr) :
    res{2} = Some ((cell_addr_to_cell Honest gm cell_addr').`cont)].
 proof.
 proc; inline*; sp 2 0.
-rcondt{1} 1; first auto.
 if => //; auto; smt().
 qed.
 
@@ -4406,7 +3958,6 @@ lemma is_cell_read_cell_bad (gm : gm, cell_addr' : addr) :
    ! res{1} /\ res{2} = None].
 proof.
 proc; inline*; sp 2 0.
-rcondt{1} 1; first auto.
 if => //; auto; smt().
 qed.
 
@@ -4420,7 +3971,8 @@ lemma real_simulator_unlock_cell_gm_invar_guesser
    ={res, glob Memory} /\ gm_invar (glob Memory){1} /\
    (res{1} <> None =>
     (exists (phys_addr : addr, cell : cell),
-    (gm_to_honest_virt_map (glob Memory){1}).[oget res{1}] = Some phys_addr /\
+    (oget (gm_to_virt_map (glob Memory){1}).[Honest]).[oget res{1}] =
+    Some phys_addr /\
     (gm_to_phys_map (glob Memory){1}).[phys_addr] = Some (Cell cell) /\
     cell.`cont = cont /\ cell.`locked = false))].
 proof.
@@ -4430,26 +3982,24 @@ conseq
    ={res, glob Memory} /\
    (res{1} <> None =>
     (exists (phys_addr : addr, cell : cell),
-    (gm_to_honest_virt_map (glob Memory){1}).[oget res{1}] = Some phys_addr /\
+    (oget (gm_to_virt_map (glob Memory){1}).[Honest]).[oget res{1}] =
+    Some phys_addr /\
     (gm_to_phys_map (glob Memory){1}).[phys_addr] = Some (Cell cell) /\
     cell.`cont = cont /\ cell.`locked = false)))
   (_ : gm_invar (glob Memory) ==> gm_invar (glob Memory))
   (_ : _ ==> _) => //.
 apply HonestMemory.party_memory_unlock_cell_gm_invar.
 proc; inline *; sp 3 3.
-rcondt{1} 1; first auto.
-rcondt{2} 1; first auto.
 if => //.
 sp 2 2.
 if => //.
 sp 2 2.
 if => //.
 auto => &1 &2 |>.
-rewrite /gm_to_honest_virt_map /gm_to_phys_map /= get_set_sameE.
+rewrite /gm_to_virt_map /gm_to_phys_map /= get_set_sameE oget_some.
+rewrite get_set_sameE /=.
 smt(get_setE).
-auto.
-auto.
-auto.
+auto. auto. auto.
 qed.
 
 type sim_honest_party_state = [
@@ -5090,22 +4640,24 @@ seq 1 1 :
    Memory.phys_map{1} =
    (gm_to_phys_map gm)
      .[gm_to_next_phys_addr gm <- Key (gm_to_next_key gm)] /\
-   Memory.honest_next_virt_addr{1} =
-   gm_to_honest_next_virt_addr gm + 1 /\
-   Memory.honest_virt_map{1} =
-   (gm_to_honest_virt_map gm)
-      .[gm_to_honest_next_virt_addr gm <- gm_to_next_phys_addr gm] /\
-   key_addr{1} = gm_to_honest_next_virt_addr gm /\
-   Memory.malicious_next_virt_addr{1} = gm_to_malicious_next_virt_addr gm /\
-   Memory.malicious_virt_map{1} = gm_to_malicious_virt_map gm /\
+   oget Memory.next_virt_addr.[Honest]{1} =
+   oget (gm_to_next_virt_addr gm).[Honest] + 1 /\
+   oget Memory.virt_map{1}.[Honest] =
+   (oget (gm_to_virt_map gm).[Honest])
+     .[oget (gm_to_next_virt_addr gm).[Honest] <- gm_to_next_phys_addr gm] /\
+   key_addr{1} = oget (gm_to_next_virt_addr gm).[Honest] /\
+   Memory.next_virt_addr{1}.[Malicious] =
+   (gm_to_next_virt_addr gm).[Malicious] /\
+   Memory.virt_map{1}.[Malicious] = (gm_to_virt_map gm).[Malicious] /\
    (forall (mal_virt_addr : addr),
-    mal_virt_addr \in gm_to_malicious_virt_map gm =>
+    mal_virt_addr \in oget (gm_to_virt_map gm).[Malicious] =>
     let phys_addr' =
-      oget (gm_to_malicious_virt_map gm).[mal_virt_addr] in
+      oget (oget (gm_to_virt_map gm).[Malicious]).[mal_virt_addr] in
     oget Memory.phys_map{1}.[phys_addr'] <> Key (gm_to_next_key gm))).
 call{1} (HonestMemory.party_memory_create_key_phl gm).
 call{2} (HonestMemory.party_memory_create_key_phl gm).
-auto; smt(gm_invar_old_mal_virt_addr_does_not_give_new_key).
+auto;
+  smt(fmap_eqP mem_fdom fdomP gm_invar_old_virt_addr_does_not_give_new_key).
 exlim (glob Memory){1}, key_addr{1}, choice{1} => gm' key_addr' choice'.
 call{1} (HonestMemory.party_memory_create_cell_phl gm' key_addr' choice').
 call{2} (HonestMemory.party_memory_create_cell_phl gm' key_addr' true).
@@ -5113,9 +4665,10 @@ auto; progress [-delta].
 smt(get_setE).
 apply
   (RI_Chooser_WaitCellAddrToOther _ _ _ _ _ choice{2}
-   (gm_to_honest_next_virt_addr gm) (gm_to_honest_next_virt_addr gm + 1)
+   (oget (gm_to_next_virt_addr gm).[Honest])
+   (oget (gm_to_next_virt_addr gm).[Honest] + 1)
    (gm_to_next_phys_addr gm + 1) (gm_to_next_key gm)).
-smt(fdom_set get_setE).
+progress; smt(get_setE fdom_set fmap_eqP mem_fdom fdomP).
 wp.
 ((match => //; first auto; smt(RI_Chooser_WaitChoiceFromAdv));
   first auto; exfalso; smt());
@@ -5255,7 +4808,7 @@ rewrite
   (RI_Chooser_WaitKeyAddrToOther _ _ _ _ _
    choice key_addr guess) /#.
 call (malicious_party_gm_invar_from_adv Malicious).
-auto; progress [-delta]; first 8 smt().
+auto; progress [-delta]; first 6 smt().
 rewrite
   (RI_Chooser_WaitKeyAddrToOther _ _ _ _ _
    choice key_addr guess) /#.
@@ -5276,7 +4829,7 @@ match IPS_Chooser_WaitToAdvResult {2} 2; first auto; smt().
 auto; progress [-delta].
 rewrite (RI_Chooser_WaitResultToAdv _ _ _ _ _ result) /#.
 call (malicious_party_gm_invar_from_adv Malicious).
-auto; progress [-delta]; first 8 smt().
+auto; progress [-delta]; first 6 smt().
 rewrite (RI_Chooser_WaitResultToAdv _ _ _ _ _ result) /#.
 (* ri_chooser_wait_error_to_adv *)
 move => invar_ri_chooser_wait_error_to_adv.
@@ -5295,7 +4848,7 @@ match IPS_Chooser_WaitToAdvError {2} 2; first auto; smt().
 auto; progress [-delta].
 rewrite RI_Chooser_WaitErrorToAdv /#.
 call (malicious_party_gm_invar_from_adv Malicious).
-auto; progress [-delta]; first 8 smt().
+auto; progress [-delta]; first 6 smt().
 rewrite RI_Chooser_WaitErrorToAdv /#.
 (* ri_chooser_final *)
 move => invar_ri_chooser_final.
@@ -5314,7 +4867,7 @@ match IPS_Chooser_Final {2} 2; first auto; smt().
 auto; progress [-delta].
 rewrite RI_Chooser_Final /#.
 call (malicious_party_gm_invar_from_adv Malicious).
-auto; progress [-delta]; first 8 smt().
+auto; progress [-delta]; first 6 smt().
 rewrite RI_Chooser_Final /#.
 (* ri_guesser_wait_guess_from_adv *)
 move => invar_ri_guesser_wait_guess_from_adv.
@@ -5345,7 +4898,7 @@ exfalso; smt().
 auto; progress [-delta].
 rewrite (RI_Guesser_WaitGuessFromAdv _ _ _ _ _) /#.
 call (malicious_party_gm_invar_from_adv Malicious).
-auto; progress [-delta]; first 8 smt().
+auto; progress [-delta]; first 6 smt().
 rewrite (RI_Guesser_WaitGuessFromAdv _ _ _ _ _) /#.
 (* ri_guesser_wait_cell_addr_from_other *)
 move => guess invar_ri_guesser_wait_cell_addr_from_other.
@@ -5365,7 +4918,7 @@ match IPS_Guesser_WaitSimChoice {2} 1; first auto; smt().
 auto; progress [-delta].
 rewrite (RI_Guesser_WaitCellAddrFromOther _ _ _ _ _ guess) /#.
 call (malicious_party_gm_invar_from_adv Malicious).
-auto; progress [-delta]; first 8 smt().
+auto; progress [-delta]; first 6 smt().
 rewrite (RI_Guesser_WaitCellAddrFromOther _ _ _ _ _ guess) /#.
 (* ri_guesser_wait_guess_to_other *)
 move =>
@@ -5392,7 +4945,7 @@ rewrite
 call
   (malicious_party_gm_invar_guesser_from_adv
    cell_addr cell_phys_addr cont Malicious).
-auto; progress [-delta]; first 9 smt().
+auto; progress [-delta]; first 7 smt().
 rewrite
   (RI_Guesser_WaitGuessToOther _ _ _ _ _
    guess cell_addr cell_phys_addr cont result) /#.
@@ -5421,7 +4974,7 @@ rewrite
 call
   (malicious_party_gm_invar_guesser_from_adv
    cell_addr cell_phys_addr cont Malicious).
-auto; progress [-delta]; first 9 smt().
+auto; progress [-delta]; first 7 smt().
 rewrite
   (RI_Guesser_WaitKeyAddrFromOther _ _ _ _ _
    guess cell_addr cell_phys_addr cont result) /#.
@@ -5443,7 +4996,7 @@ match IPS_Guesser_WaitToAdvResult {2} 1; first auto; smt().
 auto; progress [-delta].
 rewrite (RI_Guesser_WaitResultToAdv _ _ _ _ _ result) /#.
 call (malicious_party_gm_invar_from_adv Malicious).
-auto; progress [-delta]; first 8 smt().
+auto; progress [-delta]; first 6 smt().
 rewrite (RI_Guesser_WaitResultToAdv _ _ _ _ _ result) /#.
 (* ri_guesser_wait_error_to_adv *)
 move => invar_ri_guesser_wait_error_to_adv.
@@ -5463,7 +5016,7 @@ match IPS_Guesser_WaitToAdvError {2} 1; first auto; smt().
 auto; progress [-delta].
 rewrite (RI_Guesser_WaitErrorToAdv _ _ _ _ _) /#.
 call (malicious_party_gm_invar_from_adv Malicious).
-auto; progress [-delta]; first 8 smt().
+auto; progress [-delta]; first 6 smt().
 rewrite (RI_Guesser_WaitErrorToAdv _ _ _ _ _) /#.
 (* ri_guesser_final *)
 move => invar_ri_guesser_final.
@@ -5483,7 +5036,7 @@ match IPS_Guesser_Final {2} 1; first auto; smt().
 auto; progress [-delta].
 rewrite (RI_Guesser_Final _ _ _ _ _) /#.
 call (malicious_party_gm_invar_from_adv Malicious).
-auto; progress [-delta]; first 8 smt().
+auto; progress [-delta]; first 6 smt().
 rewrite (RI_Guesser_Final _ _ _ _ _) /#.
 qed.
 
@@ -5524,7 +5077,7 @@ match IPS_Chooser_WaitFromAdvChoice {2} 2; first auto; smt().
 auto; progress [-delta].
 rewrite RI_Chooser_WaitChoiceFromAdv /#.
 call (malicious_party_gm_invar_to_adv Malicious).
-auto; progress [-delta]; first 8 smt().
+auto; progress [-delta]; first 6 smt().
 rewrite RI_Chooser_WaitChoiceFromAdv /#.
 (* ri_chooser_wait_cell_addr_to_other *)
 move => choice key_addr cell_addr cell_phys_addr key
@@ -5658,7 +5211,7 @@ rewrite
   (RI_Chooser_WaitKeyAddrToOther _ _ _ _ _
    choice key_addr guess) /#.
 call (malicious_party_gm_invar_to_adv Malicious).
-auto; progress [-delta]; first 8 smt().
+auto; progress [-delta]; first 6 smt().
 rewrite
   (RI_Chooser_WaitKeyAddrToOther _ _ _ _ _
    choice key_addr guess) /#.
@@ -5679,7 +5232,7 @@ match IPS_Chooser_WaitToAdvResult {2} 2; first auto; smt().
 auto; progress [-delta]; first smt().
 rewrite RI_Chooser_Final /#.
 call (malicious_party_gm_invar_to_adv Malicious).
-auto; progress [-delta]; first 8 smt().
+auto; progress [-delta]; first 6 smt().
 rewrite (RI_Chooser_WaitResultToAdv _ _ _ _ _ result) /#.
 (* ri_chooser_wait_error_to_adv *)
 move => invar_ri_chooser_wait_error_to_adv.
@@ -5698,7 +5251,7 @@ match IPS_Chooser_WaitToAdvError {2} 2; first auto; smt().
 auto; progress [-delta].
 rewrite RI_Chooser_Final /#.
 call (malicious_party_gm_invar_to_adv Malicious).
-auto; progress [-delta]; first 8 smt().
+auto; progress [-delta]; first 6 smt().
 rewrite (RI_Chooser_WaitErrorToAdv _ _ _ _ _) /#.
 (* ri_chooser_final *)
 move => invar_ri_chooser_final.
@@ -5717,7 +5270,7 @@ match IPS_Chooser_Final {2} 2; first auto; smt().
 auto; progress [-delta].
 by rewrite RI_Chooser_Final.
 call (malicious_party_gm_invar_to_adv Malicious).
-auto; progress [-delta]; first 8 smt().
+auto; progress [-delta]; first 6 smt().
 rewrite RI_Chooser_Final /#.
 (* ri_guesser_wait_guess_from_adv *)
 move => invar_ri_guesser_wait_guess_from_adv.
@@ -5736,7 +5289,7 @@ match IPS_Guesser_WaitFromAdvGuess {2} 2; first auto; smt().
 auto; progress [-delta].
 rewrite RI_Guesser_WaitGuessFromAdv /#.
 call (malicious_party_gm_invar_to_adv Malicious).
-auto; progress [-delta]; first 8 smt().
+auto; progress [-delta]; first 6 smt().
 rewrite RI_Guesser_WaitGuessFromAdv /#.
 (* ri_guesser_wait_cell_addr_from_other *)
 move => guess invar_ri_guesser_wait_cell_addr_from_other.
@@ -5755,7 +5308,7 @@ match IPS_Guesser_WaitSimChoice {2} 2; first auto; smt().
 auto; progress [-delta].
 rewrite (RI_Guesser_WaitCellAddrFromOther _ _ _ _ _ guess) /#.
 call (malicious_party_gm_invar_to_adv Malicious).
-auto; progress [-delta]; first 8 smt().
+auto; progress [-delta]; first 6 smt().
 rewrite (RI_Guesser_WaitCellAddrFromOther _ _ _ _ _ guess) /#.
 (* ri_guesser_wait_guess_to_other *)
 move =>
@@ -5781,7 +5334,7 @@ rewrite
 call
   (malicious_party_gm_invar_guesser_to_adv
    cell_addr cell_phys_addr cont Malicious).
-auto; progress [-delta]; first 9 smt().
+auto; progress [-delta]; first 7 smt().
 rewrite
   (RI_Guesser_WaitGuessToOther _ _ _ _ _
    guess cell_addr cell_phys_addr cont result) /#.
@@ -5809,7 +5362,7 @@ rewrite
 call
   (malicious_party_gm_invar_guesser_to_adv
    cell_addr cell_phys_addr cont Malicious).
-auto; progress [-delta]; first 9 smt().
+auto; progress [-delta]; first 7 smt().
 rewrite
   (RI_Guesser_WaitKeyAddrFromOther _ _ _ _ _
    guess cell_addr cell_phys_addr cont result) /#.
@@ -5830,7 +5383,7 @@ match IPS_Guesser_WaitToAdvResult {2} 2; first auto; smt().
 auto; progress [-delta]; first smt().
 rewrite RI_Guesser_Final /#.
 call (malicious_party_gm_invar_to_adv Malicious).
-auto; progress [-delta]; first 8 smt().
+auto; progress [-delta]; first 6 smt().
 rewrite (RI_Guesser_WaitResultToAdv _ _ _ _ _ result) /#.
 (* ri_guesser_wait_error_to_adv *)
 move => invar_ri_guesser_wait_error_to_adv.
@@ -5849,7 +5402,7 @@ match IPS_Guesser_WaitToAdvError {2} 2; first auto; smt().
 auto; progress [-delta].
 rewrite (RI_Guesser_Final _ _ _ _ _) /#.
 call (malicious_party_gm_invar_to_adv Malicious).
-auto; progress [-delta]; first 8 smt().
+auto; progress [-delta]; first 6 smt().
 rewrite RI_Guesser_WaitErrorToAdv /#.
 (* ri_guesser_final *)
 move => invar_ri_guesser_final.
@@ -5868,7 +5421,7 @@ match IPS_Guesser_Final {2} 2; first auto; smt().
 auto; progress [-delta].
 rewrite RI_Guesser_Final /#.
 call (malicious_party_gm_invar_to_adv Malicious).
-auto; progress [-delta]; first 8 smt().
+auto; progress [-delta]; first 6 smt().
 rewrite RI_Guesser_Final /#.
 qed.
 
@@ -5916,7 +5469,7 @@ by rewrite RI_Chooser_WaitChoiceFromAdv.
 inline Simulator(Malicious).malicious_queue.
 wp.
 call (malicious_party_gm_invar_to_other Malicious).
-auto; progress [-delta]; first 8 smt().
+auto; progress [-delta]; first 6 smt().
 rewrite RI_Chooser_WaitChoiceFromAdv /#.
 (* ri_chooser_wait_cell_addr_to_other *)
 move => choice' key_addr' cell_addr' cell_phys_addr' key'
@@ -6096,7 +5649,7 @@ rewrite (RI_Chooser_WaitResultToAdv _ _ _ _ _ result{2}) /#.
 inline Simulator(Malicious).malicious_queue.
 wp.
 call (malicious_party_gm_invar_to_other Malicious).
-auto; progress [-delta]; first 8 smt().
+auto; progress [-delta]; first 6 smt().
 rewrite
   (RI_Chooser_WaitKeyAddrToOther _ _ _ _ _
    choice' key_addr' guess') /#.
@@ -6121,7 +5674,7 @@ rewrite (RI_Chooser_WaitResultToAdv _ _ _ _ _ result') /#.
 inline Simulator(Malicious).malicious_queue.
 wp.
 call (malicious_party_gm_invar_to_other Malicious).
-auto; progress [-delta]; first 8 smt().
+auto; progress [-delta]; first 6 smt().
 rewrite (RI_Chooser_WaitResultToAdv _ _ _ _ _ result') /#.
 (* ri_chooser_wait_error_to_adv *)
 move => invar_ri_chooser_wait_error_to_adv.
@@ -6144,7 +5697,7 @@ rewrite RI_Chooser_WaitErrorToAdv /#.
 inline Simulator(Malicious).malicious_queue.
 wp.
 call (malicious_party_gm_invar_to_other Malicious).
-auto; progress [-delta]; first 8 smt().
+auto; progress [-delta]; first 6 smt().
 rewrite (RI_Chooser_WaitErrorToAdv _ _ _ _ _) /#.
 (* ri_chooser_final *)
 move => invar_ri_chooser_final.
@@ -6168,7 +5721,7 @@ by rewrite RI_Chooser_Final.
 inline Simulator(Malicious).malicious_queue.
 wp.
 call (malicious_party_gm_invar_to_other Malicious).
-auto; progress [-delta]; first 8 smt().
+auto; progress [-delta]; first 6 smt().
 rewrite RI_Chooser_Final /#.
 (* ri_guesser_wait_guess_from_adv *)
 move => invar_ri_guesser_wait_guess_from_adv.
@@ -6192,7 +5745,7 @@ by rewrite RI_Guesser_WaitGuessFromAdv.
 inline Simulator(Malicious).malicious_queue.
 wp.
 call (malicious_party_gm_invar_to_other Malicious).
-auto; progress [-delta]; first 8 smt().
+auto; progress [-delta]; first 6 smt().
 rewrite RI_Guesser_WaitGuessFromAdv /#.
 (* ri_guesser_wait_cell_addr_from_other *)
 move => guess' invar_ri_guesser_wait_cell_addr_from_other.
@@ -6216,7 +5769,7 @@ rewrite (RI_Guesser_WaitCellAddrFromOther _ _ _ _ _ guess') /#.
 inline Simulator(Malicious).malicious_queue.
 wp.
 call (malicious_party_gm_invar_to_other Malicious).
-auto; progress [-delta]; first 8 smt().
+auto; progress [-delta]; first 6 smt().
 rewrite (RI_Guesser_WaitCellAddrFromOther _ _ _ _ _ guess') /#.
 (* ri_guesser_wait_guess_to_other *)
 move =>
@@ -6247,7 +5800,7 @@ wp.
 call
   (malicious_party_gm_invar_guesser_to_other cell_addr'
    cell_phys_addr' cont' Malicious).
-auto; progress [-delta]; first 9 smt().
+auto; progress [-delta]; first 7 smt().
 rewrite
   (RI_Guesser_WaitGuessToOther _ _ _ _ _
    guess' cell_addr' cell_phys_addr' cont' result') /#.
@@ -6280,7 +5833,7 @@ wp.
 call
   (malicious_party_gm_invar_guesser_to_other cell_addr'
    cell_phys_addr' cont' Malicious).
-auto; progress [-delta]; first 9 smt().
+auto; progress [-delta]; first 7 smt().
 rewrite
   (RI_Guesser_WaitKeyAddrFromOther _ _ _ _ _
    guess' cell_addr' cell_phys_addr' cont' result') /#.
@@ -6306,7 +5859,7 @@ rewrite (RI_Guesser_WaitResultToAdv _ _ _ _ _ result') /#.
 inline Simulator(Malicious).malicious_queue.
 wp.
 call (malicious_party_gm_invar_to_other Malicious).
-auto; progress [-delta]; first 8 smt().
+auto; progress [-delta]; first 6 smt().
 rewrite (RI_Guesser_WaitResultToAdv _ _ _ _ _ result') /#.
 (* ri_guesser_wait_error_to_adv *)
 move => invar_ri_guesser_wait_error_to_adv.
@@ -6330,7 +5883,7 @@ by rewrite RI_Guesser_WaitErrorToAdv.
 inline Simulator(Malicious).malicious_queue.
 wp.
 call (malicious_party_gm_invar_to_other Malicious).
-auto; progress [-delta]; first 8 smt().
+auto; progress [-delta]; first 6 smt().
 rewrite RI_Guesser_WaitErrorToAdv /#.
 (* ri_guesser_final *)
 move => invar_ri_guesser_final.
@@ -6354,7 +5907,7 @@ by rewrite RI_Guesser_Final.
 inline Simulator(Malicious).malicious_queue.
 wp.
 call (malicious_party_gm_invar_to_other Malicious).
-auto; progress [-delta]; first 8 smt().
+auto; progress [-delta]; first 6 smt().
 rewrite RI_Guesser_Final /#.
 qed.
 
@@ -6412,7 +5965,7 @@ by rewrite RI_Chooser_WaitChoiceFromAdv.
 move => msg1 msgs1 msg2 msgs2.
 wp.
 call (malicious_party_gm_invar_from_other Malicious).
-(auto; progress [-delta]; first 8 smt());
+(auto; progress [-delta]; first 6 smt());
   rewrite RI_Chooser_WaitChoiceFromAdv /#.
 (* ri_chooser_wait_cell_addr_to_other *)
 move => choice' key_addr' cell_addr' cell_phys_addr' key'
@@ -6675,7 +6228,7 @@ rewrite
 move => msg1 msgs1 msg2 msgs2.
 wp.
 call (malicious_party_gm_invar_from_other Malicious).
-(auto; progress [-delta]; first 8 auto; smt());
+(auto; progress [-delta]; first 6 auto; smt());
   rewrite
     (RI_Chooser_WaitKeyAddrToOther _ _ _ _ _
      choice' key_addr' guess') /#.
@@ -6712,7 +6265,7 @@ rewrite (RI_Chooser_WaitResultToAdv _ _ _ _ _ result') /#.
 move => msg1 msgs1 msg2 msgs2.
 wp.
 call (malicious_party_gm_invar_from_other Malicious).
-auto; progress [-delta]; first 8 auto; smt().
+auto; progress [-delta]; first 6 auto; smt().
 rewrite (RI_Chooser_WaitResultToAdv _ _ _ _ _ result') /#.
 rewrite (RI_Chooser_WaitResultToAdv _ _ _ _ _ result') /#.
 (* ri_chooser_wait_error_to_adv *)
@@ -6748,7 +6301,7 @@ by rewrite RI_Chooser_WaitErrorToAdv.
 move => msg1 msgs1 msg2 msgs2.
 wp.
 call (malicious_party_gm_invar_from_other Malicious).
-auto; progress [-delta]; first 8 smt().
+auto; progress [-delta]; first 6 smt().
 rewrite (RI_Chooser_WaitErrorToAdv _ _ _ _ _) /#.
 rewrite (RI_Chooser_WaitErrorToAdv _ _ _ _ _) /#.
 (* ri_chooser_final *)
@@ -6784,7 +6337,7 @@ by rewrite RI_Chooser_Final.
 move => msg1 msgs1 msg2 msgs2.
 wp.
 call (malicious_party_gm_invar_from_other Malicious).
-(auto; progress [-delta]; first 8 smt());
+(auto; progress [-delta]; first 6 smt());
   rewrite (RI_Chooser_Final _ _ _ _ _) /#.
 (* ri_guesser_wait_guess_from_adv *)
 move => invar_ri_guesser_wait_guess_from_adv.
@@ -6819,7 +6372,7 @@ by rewrite RI_Guesser_WaitGuessFromAdv.
 move => msg1 msgs1 msg2 msgs2.
 wp.
 call (malicious_party_gm_invar_from_other Malicious).
-(auto; progress [-delta]; first 8 smt());
+(auto; progress [-delta]; first 6 smt());
   rewrite (RI_Guesser_WaitGuessFromAdv _ _ _ _ _) /#.
 (* ri_guesser_wait_cell_addr_from_other *)
 move => guess' invar_ri_guesser_wait_cell_addr_from_other.
@@ -6875,8 +6428,10 @@ auto; progress [-delta].
 pose cell := cell_addr_to_cell Honest (glob Memory){1} cell_addr{2}.
 rewrite
   (RI_Guesser_WaitGuessToOther _ _ _ _ _
-   guess{1} cell_addr{2} (oget Memory.honest_virt_map{1}.[cell_addr{2}])
-   cell.`cont (guess{2} = cell.`cont)); smt(get_some).
+   guess{1} cell_addr{2}
+   (oget (oget Memory.virt_map{1}.[Honest]).[cell_addr{2}])
+   cell.`cont (guess{2} = cell.`cont)).
+progress; smt(get_some).
 seq 1 1 : (#pre /\ ! b0{1} /\ choice_opt{2} = None).
 exlim (glob Memory){1}, cell_addr{1} => gm cell_addr'.
 call (is_cell_read_cell_bad gm cell_addr').
@@ -6905,7 +6460,7 @@ rewrite (RI_Guesser_WaitCellAddrFromOther _ _ _ _ _ guess') /#.
 move => msg1 msgs1 msg2 msgs2.
 wp.
 call (malicious_party_gm_invar_from_other Malicious).
-(auto; progress [-delta]; first 8 smt());
+(auto; progress [-delta]; first 6 smt());
   rewrite (RI_Guesser_WaitCellAddrFromOther _ _ _ _ _ guess') /#.
 (* ri_guesser_wait_guess_to_other *)
 move =>
@@ -6951,7 +6506,7 @@ wp.
 call
   (malicious_party_gm_invar_guesser_from_other
    cell_addr' cell_phys_addr' cont' Malicious).
-(auto; progress [-delta]; first 9 smt());
+(auto; progress [-delta]; first 7 smt());
   rewrite
     (RI_Guesser_WaitGuessToOther _ _ _ _ _
      guess' cell_addr' cell_phys_addr' cont' result') /#.
@@ -6998,8 +6553,8 @@ seq 1 1 :
    result' = (guess' = cont') /\
    (unlocked_cell_addr_opt{1} <> None =>
     (exists (phys_addr : addr, cell : cell),
-    (gm_to_honest_virt_map
-     (glob Memory){1}).[oget unlocked_cell_addr_opt{1}] = Some phys_addr /\
+     (oget (gm_to_virt_map (glob Memory){1}).[Honest])
+        .[oget unlocked_cell_addr_opt{1}] = Some phys_addr /\
     (gm_to_phys_map (glob Memory){1}).[phys_addr] = Some (Cell cell) /\
     cell.`cont = cont' /\ cell.`locked = false))).
 call
@@ -7052,7 +6607,7 @@ wp.
 call
   (malicious_party_gm_invar_guesser_from_other
    cell_addr' cell_phys_addr' cont' Malicious).
-(auto; progress [-delta]; first 9 smt());
+(auto; progress [-delta]; first 7 smt());
   rewrite
     (RI_Guesser_WaitKeyAddrFromOther _ _ _ _ _
      guess' cell_addr' cell_phys_addr' cont' result') /#.
@@ -7087,7 +6642,7 @@ rewrite (RI_Guesser_WaitResultToAdv _ _ _ _ _ result') /#.
 move => msg1 msgs1 msg2 msgs2.
 wp.
 call (malicious_party_gm_invar_from_other Malicious).
-(auto; progress [-delta]; first 8 smt());
+(auto; progress [-delta]; first 6 smt());
   rewrite (RI_Guesser_WaitResultToAdv _ _ _ _ _ result') /#.
 (* ri_guesser_wait_error_to_adv *)
 move => invar_ri_guesser_wait_error_to_adv.
@@ -7120,7 +6675,7 @@ by rewrite RI_Guesser_WaitErrorToAdv.
 move => msg1 msgs1 msg2 msgs2.
 wp.
 call (malicious_party_gm_invar_from_other Malicious).
-(auto; progress [-delta]; first 8 smt());
+(auto; progress [-delta]; first 6 smt());
   rewrite (RI_Guesser_WaitErrorToAdv _ _ _ _ _) /#.
 (* ri_guesser_final *)
 move => invar_ri_guesser_final.
@@ -7153,7 +6708,7 @@ by rewrite RI_Guesser_Final.
 move => msg1 msgs1 msg2 msgs2.
 wp.
 call (malicious_party_gm_invar_from_other Malicious).
-(auto; progress [-delta]; first 8 smt());
+(auto; progress [-delta]; first 6 smt());
   rewrite (RI_Guesser_Final _ _ _ _ _) /#.
 qed.
 
@@ -7211,8 +6766,9 @@ qed.
 
 end section.
 
-(* we have perfect security: the adversary has no chance of
-   distinguishing the real and ideal worlds
+(* we have perfect security: the probability that Adv returns true in
+   the real experiment is exactly the same as the probability it
+   returns true in the ideal experiment
 
    assuming we resrict ourselves to Malicious and Adv being
    non-probabilistic, we can conclude that the real experiment results
