README.md
@@ -1,16 +1,21 @@
-Formalization of a Two-party Guessing Game in EasyCrypt
-=======================================================
+Security Through Indirection of a Two-party Guessing Game in EasyCrypt
+======================================================================
 
 This repository contains the formalization in
 [EasyCrypt](https://github.com/EasyCrypt/easycrypt) of a two-party
-guessing game and the proof of its security in a real/ideal
-style. Security is achieved by relying not on cryptographic
-mechanisms, but on a shared trusted infrastructure in which immutable
-objects are stored in a physical memory, and the two parties have
-virtual memories giving them indirect access to certain objects.
+boolean guessing game, together with the definition and proof of the
+security of an honest party against a possibly malicious one in a
+real/ideal simulation-based style. Security is achieved by relying not
+on cryptographic mechanisms, but on a shared trusted computing base in
+which immutable objects are stored in a physical memory, and the two
+parties have virtual memories giving them indirect access to certain
+objects. We call this "security through indirection". Correctness of
+the protocol is also proved, assuming both parties are honest.
 
-This work is part of a collaboration between
+This work is part of a collaboration between myself
+([Alley Stoughton](https://alleystoughton.us))
+and
 [Arthur Azevedo de Amorim](https://arthuraa.net),
-[Marco Gaboardi](https://cs-people.bu.edu/gaboardi/),
-[Jared Pincus](https://jaredpincus.com) and
-[Alley Stoughton](https://alleystoughton.us).
+[Marco Gaboardi](https://cs-people.bu.edu/gaboardi/) and
+[Jared Pincus](https://jaredpincus.com).
+
